backend/Scheduling.v
@@ -1,5 +1,3008 @@
+(* Require Import ExtrOcamlIntConv.
+Parameter prioritizer : list int -> int -> list (list int) -> int -> unit. *)
+
+
+Require Import Globalenvs Events Smallstep.
+Section SMALL_STEP_EXT.
+  Variable L: Smallstep.semantics.
+
+  Theorem forward_simulation_refl: forward_simulation L L.
+  Proof.
+    eapply forward_simulation_step with (match_states := eq).
+    auto. intros; eauto. intros; subst; auto.
+    intros; subst; eauto.
+  Qed. 
+
+End SMALL_STEP_EXT.
+
+
+Require Import Coqlib Maps BoolEqual.
+
+Import ListNotations.
+Open Scope list_scope.
+Open Scope nat_scope.
+
+Require Import List Lia.
+
+Section LIST_INDUCTION.  
+  Variable A : Type.
+  Variable P : list A -> Prop.
+  Hypothesis H : forall xs, (forall l, length l < length xs -> P l) -> P xs.
+
+  Theorem list_length_ind : forall xs, P xs.
+  Proof.
+    assert (forall xs l : list A, length l <= length xs -> P l) as H_ind.
+    { induction xs; intros l Hlen; apply H; intros l0 H0.
+      - inversion Hlen. lia.
+      - apply IHxs. simpl in Hlen. lia. }
+    intros xs. apply H_ind with (xs := xs). lia.
+  Qed.
+End LIST_INDUCTION.
+
+
+(** TODO: move to TopoSort files *)
+Open Scope nat_scope.
+Require Import Relations.Relation_Definitions.
+Section TRY_SWAP.
+
+  Context {A: Type}.
+  Variable (rel: A -> A -> bool).
+
+  Fixpoint try_swap (n: nat) (l: list A): list A :=
+    match n, l with
+    | _, nil => nil | _, i :: nil => l        (* None: did not swap *)
+    | O, i1 :: i2 :: l' => if rel i1 i2 then l
+                           else (i2 :: i1 :: l')
+    | Datatypes.S n', i :: l' => i :: try_swap n' l'
+    end.
+  
+  (* Lemma try_swap_later: 
+    forall (n:nat) l a, 0 < n -> try_swap n (a :: l) = a :: try_swap (n-1) l.
+  Proof. Admitted. *)
+
+  Lemma try_swap_nil: forall n, try_swap n [] = [].
+  Proof. intros; destruct n; auto. Qed.
+
+  Lemma try_swap_singleton: forall n x, try_swap n ([x]) = [x].
+  Proof. intros n. induction n; simpl; auto. Qed.
+
+  Lemma try_swap_at_tail: forall l, try_swap (length l) l = l.
+  Proof.
+    assert(try_swap_at_tail_aux: forall l a, 
+      try_swap (length (a::l)) (a::l) = a :: try_swap (length l) l ).
+    { induction l; intros. simpl; auto. simpl. rewrite <- IHl; auto. }
+    induction l. simpl; auto.
+    rewrite try_swap_at_tail_aux. rewrite IHl; auto.
+  Qed.
+
+  Lemma try_swap_head_not_change:
+    forall n x l l', try_swap n (x :: l) = x :: l' -> 
+        exists n', try_swap n' l = l'.
+  Proof.
+    intros. destruct n; simpl in H.
+    - destruct l. inv H. exists O; auto. eexists (length (a :: l)). 
+      destruct (rel x a); inv H; eapply try_swap_at_tail.
+    - destruct l. inv H. exists O; auto. inv H. exists n; auto.
+  Qed.
+
+  Fixpoint try_swap_seq (ln: list nat) (la: list A): list A :=
+    match ln with
+    | nil => la
+    | n :: ln' => try_swap_seq ln' (try_swap n la)
+    end.
+
+  Lemma try_swap_seq_nil: forall ln, try_swap_seq ln [] = [].
+  Proof. induction ln; simpl; auto. rewrite try_swap_nil; auto. Qed.
+
+  Lemma try_swap_seq_singleton: forall ln x, try_swap_seq ln [x] = [x].
+  Proof. induction ln; simpl; auto. intros. rewrite try_swap_singleton; auto. Qed.
+
+  Lemma try_swap_app: forall ln1 ln2 l,
+    try_swap_seq (ln1 ++ ln2) l = try_swap_seq ln2 (try_swap_seq ln1 l).
+  Proof. induction ln1; intros; simpl; auto. Qed.
+
+End TRY_SWAP.
+
+
+
+
+
+
+Require Import Sorting.Permutation.
+Section TOPO_REORDER.
+
+  Context {A: Type}.
+
+  (* exactly same elements *)
+  Inductive NoDupSame: list A -> list A -> Prop :=
+  | NoDupSame_intro:
+    forall l1 l2, NoDup l1 -> NoDup l2 -> incl l1 l2 -> incl l2 l1 ->
+      NoDupSame l1 l2
+  .
+  
+  Theorem SameLength_NoDupSame:
+    forall l1 l2, length l1 = length l2 -> NoDup l1 -> NoDup l2 -> incl l2 l1 -> NoDupSame l1 l2.
+  Proof. 
+    intros. eapply NoDupSame_intro; auto.
+    intro; intros. inv H0. destruct H3. 
+  Admitted.   
+
+
+  Variable R: A -> A -> Prop.
+
+  (* Inductive sublist: list A -> list A -> Prop :=
+  | sublist_refl: forall l, sublist l l
+  | sublist_rm: forall l l1 a l2, sublist (l1 ++ [a] ++ l2) l -> sublist (l1 ++ l2) l   
+  .
+
+  Lemma sublist_nil_all: forall l, sublist [] l.
+  Proof. induction l; intros. apply sublist_refl. 
+  Admitted.
+
+  Lemma sublist_same_length:
+    forall l' l, sublist l' l -> length l = length l' -> l = l'.
+  Proof.
+    induction l'. intros.
+    - admit.
+    - intros. destruct l.
+      + admit.
+      + 
+  Admitted. *)
+
+  (* not greater than any elements in list *)
+  Inductive ngt (a: A): list A -> Prop :=
+  | ngt_nil: ngt a []
+  | ngt_l: forall x, ~ R x a -> ngt a [x]  (* TODO: delete this redundant constructor *)
+  | ngt_cons: forall x l, ngt a l -> ~ R x a -> ngt a (x :: l)  
+  .
+
+  (* equivlent definition *)
+  Definition ngt' (a: A) (l: list A) := forall x, In x l  -> ~ R x a.
+
+  Lemma ngt_ngt': forall l a, ngt a l -> ngt' a l.
+  Proof.
+    induction l; intros; simpl. intro; intros. intro; auto.
+    inv H. intro; intros. destruct H; subst; auto.
+    eapply IHl in H2. intro; intros. destruct H; subst; auto.
+  Qed.
+
+  Lemma ngt'_ngt: forall l a, ngt' a l -> ngt a l.
+  Proof.
+    induction l; intros. apply ngt_nil.
+    apply ngt_cons. eapply IHl. unfold ngt' in H.
+    intro; intros. eapply H. right; auto.
+    apply H; left; auto.
+  Qed.
+
+  Inductive topo_sorted: list A -> Prop :=
+  | topo_sorted_nil: topo_sorted []
+  (* | topo_sorted_l: forall x, topo_sorted [x] *)
+  | topo_sorted_cons: forall x l, ngt x l -> topo_sorted l -> topo_sorted (x :: l)
+  .
+
+  Inductive topo_reorder : list A -> list A -> Prop :=
+  | topo_reorder_nil: topo_reorder [] []
+  | topo_reorder_skip x l l' : ngt x l -> topo_reorder l l' -> topo_reorder (x::l) (x::l')
+  | topo_reorder_swap x y l : (~ R x y) -> (~ R y x) -> topo_reorder (y::x::l) (x::y::l)
+  | topo_reorder_trans l l' l'' :
+      topo_reorder l l' -> topo_reorder l' l'' -> topo_reorder l l''.
+
+  Inductive topo_reorder' : list A -> list A -> Prop :=
+  | topo_reorder_nil': topo_reorder' [] []
+  | topo_reorder_single': forall x, topo_reorder' [x] [x]
+  | topo_reorder_swap' x y l1 l2 : ~ R x y -> ~ R y x -> topo_reorder' (l1 ++ (y::x::l2)) (l1 ++ (x::y::l2)).
+  (* | topo_reorder_trans l l' l'' :
+      topo_reorder l l' -> topo_reorder l' l'' -> topo_reorder l l''. *)
+
+  Lemma incl_nil: forall l: list A, incl l [] -> l = [].
+  Proof.
+    induction l; intros; auto.
+    assert(In a []). apply H; left; auto. exfalso; auto.
+  Qed.
+
+  Lemma ngt_cons_inv: forall x x0 l, ngt x (x0 :: l) -> ngt x l /\ ~ R x0 x.
+  Proof.
+    intros. inversion H.
+    - subst. split; auto. apply ngt_nil.
+    - subst. auto.
+  Qed.
+
+  Lemma ngt_app_inv_l: forall x l1 l2, ngt x (l1 ++ l2) -> ngt x l1.
+  Proof.
+    induction l1; intros. eapply ngt_nil.
+    inv H. eapply ngt_cons; eauto.
+    symmetry in H2; eapply app_eq_nil in H2 as []; subst. eapply ngt_nil.
+    eapply ngt_cons; eauto.
+  Qed.
+
+  Lemma ngt_app_inv_r: forall x l1 l2, ngt x (l1 ++ l2) -> ngt x l2.
+  Proof.
+    induction l1; intros; auto. eapply IHl1.
+    eapply ngt_cons_inv; eauto.
+  Qed.
+
+  Lemma ngt_app: forall x l1 l2, ngt x l1 -> ngt x l2 -> ngt x (l1 ++ l2).
+  Proof.
+    induction l1; intros; auto.
+    simpl; eapply ngt_cons. eapply IHl1; eauto.
+    eapply ngt_cons_inv; eauto. eapply ngt_cons_inv; eauto.
+  Qed.
+
+  (* Lemma topo_reorder_is_permutation: forall l l', topo_reorder l l' -> Permutation l l'.
+  Proof.
+    intros. induction H. apply perm_nil. apply perm_skip; auto.
+    - apply perm_swap. - eapply perm_trans; eauto.
+  Qed. *)
+
+  Lemma topo_reorder_incl: forall l l', topo_reorder l l' -> List.incl l l'.
+  Proof.
+    intros. induction H.
+    - apply incl_refl. - apply incl_cons. left; auto. right; auto.
+    - apply incl_cons. right. left; auto. intro; intro. destruct H1. 
+      subst. left; auto. right; right; auto.
+    - eapply incl_tran; eauto.
+  Qed.
+
+  Lemma topo_reorder_ngt_preserved:
+    forall x l l', topo_reorder l l' -> ngt x l -> ngt x l'.
+  Proof.
+    intros. induction H. - apply ngt_nil.
+    - apply ngt_cons_inv in H0 as []; auto. eapply ngt_cons; auto.
+    - inv H0. inv H4. eapply ngt_cons; auto. eapply ngt_cons; auto. eapply ngt_nil.
+      eapply ngt_cons; auto. eapply ngt_cons; auto.
+    - eapply IHtopo_reorder1 in H0. eapply IHtopo_reorder2 in H0. auto.
+  Qed.
+
+  Lemma topo_sorted_single: forall x, topo_sorted [x].
+  Proof. intros. eapply topo_sorted_cons. eapply ngt_nil. eapply topo_sorted_nil. Qed.
+
+  Lemma topo_sorted_cons_inv1:
+    forall x l, topo_sorted (x :: l) -> ngt x l.
+  Proof. intros. inv H. auto. Qed.
+
+  Lemma topo_sorted_cons_inv2:
+    forall x l, topo_sorted (x :: l) -> topo_sorted l.
+  Proof. intros. inv H. auto. Qed.
+
+  Lemma topo_sorted_split_l:
+    forall l1 l2, topo_sorted (l1 ++ l2) -> topo_sorted l1.
+  Proof.
+    induction l1. intros. eapply topo_sorted_nil.
+    intros. eapply topo_sorted_cons. inv H. eapply ngt_app_inv_l; eauto.
+    inv H. eapply IHl1; eauto.
+  Qed.
+
+  Lemma topo_sorted_split_r:
+    forall l1 l2, topo_sorted (l1 ++ l2) -> topo_sorted l2.
+  Proof.
+    induction l1. intros. simpl; auto.
+    intros. eapply IHl1. eapply topo_sorted_cons_inv2; eauto.
+  Qed.
+
+  Lemma topo_sorted_remove: forall l1 a l2, topo_sorted (l1 ++ a :: l2) -> topo_sorted (l1 ++ l2).
+  Proof.
+    induction l1; intros.
+    - simpl in *. eapply topo_sorted_cons_inv2; eauto.
+    - simpl in H. eapply topo_sorted_cons_inv1 in H as ?.
+      eapply topo_sorted_cons_inv2 in H as ?. simpl; eapply topo_sorted_cons; eauto.
+      eapply ngt_app. eapply ngt_app_inv_l; eauto.
+      eapply ngt_app_inv_r in H0. eapply ngt_cons_inv; eauto.
+  Qed.
+
+  Lemma topo_soerted_app: forall l x, topo_sorted l -> 
+    (forall a, In a l -> ~ R x a) -> topo_sorted (l ++ [x]).
+  Proof.
+    induction l; intros. simpl. eapply topo_sorted_single.
+    simpl. eapply topo_sorted_cons. eapply ngt_app.
+    inv H; auto. eapply ngt_cons. eapply ngt_nil.
+    eapply H0; left; auto. eapply IHl. eapply topo_sorted_cons_inv2; eauto.
+    intros. eapply H0. right; auto.
+  Qed.
+
+  Lemma topo_reorder_sort_preserved:
+    forall l l', topo_reorder l l' -> topo_sorted l ->  topo_sorted l'.
+  Proof.
+    intros. induction H; simpl; auto.
+    - eapply topo_sorted_cons_inv1 in H0 as ?.
+      eapply topo_sorted_cons_inv2 in H0 as ?.
+      eapply topo_sorted_cons.
+      eapply topo_reorder_ngt_preserved; eauto. eapply IHtopo_reorder; auto.
+    - inv H0. inv H5. eapply topo_sorted_cons. eapply ngt_cons; auto.
+      eapply topo_sorted_cons; eauto. eapply ngt_cons_inv; eauto.
+  Qed.
+
+  Lemma topo_reorder_cond_refl: forall l, topo_sorted l -> topo_reorder l l.
+  Proof.
+    induction l; intros. apply topo_reorder_nil.
+    inv H. eapply topo_reorder_skip; auto.
+  Qed.
+
+  Lemma topo_reorder_app: forall l1 l2 l, topo_sorted (l1 ++ l) ->
+    topo_reorder l1 l2 ->  topo_reorder (l1 ++ l) (l2 ++ l).
+  Proof.
+    intros. induction H0.
+    - eapply topo_reorder_cond_refl; auto.
+    - simpl in H. eapply topo_sorted_cons_inv1 in H as ?.
+      eapply topo_sorted_cons_inv2 in H as ?.
+      simpl. eapply topo_reorder_skip; auto.
+    - simpl. eapply topo_reorder_swap; auto.
+    - eapply IHtopo_reorder1 in H as ?.
+      eapply topo_reorder_sort_preserved in H0 as ?; eauto.
+      eapply IHtopo_reorder2 in H1. eapply topo_reorder_trans; auto.
+  Qed.
+
+  Lemma topo_reorder_symmetry: forall l l', topo_reorder l l' -> topo_reorder l' l.
+  Proof.
+    intros. induction H.
+    - apply topo_reorder_nil.
+    - apply topo_reorder_skip; auto. eapply topo_reorder_ngt_preserved; eauto.
+    - apply topo_reorder_swap; auto.
+    - eapply topo_reorder_trans; eauto. 
+  Qed.
+
+  Lemma topo_reorder_tail_to_head:
+    forall l a, topo_sorted (l ++ [a]) -> topo_sorted (a :: l) ->
+      ngt a l -> topo_reorder (l ++ [a]) (a :: l).
+  Proof.
+    induction l; intros; simpl.
+    - eapply topo_reorder_skip; auto. eapply topo_reorder_nil.
+    - eapply ngt_cons_inv in H1 as []. eapply IHl in H1 as ?.
+      assert(topo_reorder (a0 :: a :: l) (a :: a0 :: l)).
+      { simpl in H. inv H. eapply ngt_app_inv_r in H6.
+        inv H6; auto. eapply topo_reorder_swap; auto.
+        eapply topo_reorder_swap; auto. }
+      simpl in H. eapply topo_reorder_symmetry; eauto.
+      assert(topo_reorder (a :: a0 :: l) (a :: l ++ [a0])).
+      { eapply topo_reorder_skip. inv H. eapply ngt_cons.
+        eapply ngt_app_inv_l; eauto. 
+        eapply ngt_app_inv_r in H7; inv H7; eauto.
+        eapply topo_reorder_symmetry; auto.
+      }
+      eapply topo_reorder_trans; eauto.
+      replace ((a :: l) ++ [a0]) with ([a] ++ (l ++ [a0])) in H; auto.
+      eapply topo_sorted_split_r; eauto.
+      eapply topo_sorted_cons. inv H0. inv H5; auto.
+      eapply topo_sorted_cons_inv2. eapply topo_sorted_cons_inv2; eauto.
+  Qed.
+  
+
+
+
+
+  Lemma NoDupSame_nil: forall l, NoDupSame [] l -> l = [].
+  Proof. induction l; intros; auto. inv H. apply incl_nil; eauto. Qed.
+
+  (* Lemma list_common_head_split: forall l1 l2: list A,
+    exists lh l1' l2', l1 = lh ++ l1' /\ l2 = lh ++ l2'.
+  Proof. exists [], l1, l2. simpl. auto. Qed. *)
+    (* induction l1. intros.
+    - exists [], [], l2. split; auto.
+    - exist intros. eapply IHl1 in H as [lh [l1' [l2' [? []]]]].
+      subst. exists (a :: lh), l1', l2'. split; auto.
+  Admitted. *)
+
+
+  Lemma incl_remove: forall (a: A) l1 l2 l1' l2', NoDup (l1 ++ a :: l2) ->
+    incl (l1 ++ a :: l2) (l1' ++ a :: l2') -> incl (l1 ++ l2) (l1' ++ l2').
+  Proof.
+    intros. intro. intros. eapply in_or_app. eapply in_app_or in H1. destruct H1.
+    assert(a0 <> a). eapply NoDup_remove in H as [].
+    intro; subst. apply H2. apply in_or_app; eauto. 
+    assert(In a0 (l1' ++ a :: l2')). eapply H0. apply in_or_app; auto.
+    apply in_app_or in H3. destruct H3; auto. destruct H3; auto.
+    exfalso; apply H2; auto.
+    assert(a0 <> a). eapply NoDup_remove in H as [].
+    intro; subst. apply H2. apply in_or_app; eauto. 
+    assert(In a0 (l1' ++ a :: l2')). eapply H0.
+    apply in_or_app; right; right; auto.
+    apply in_app_or in H3. destruct H3; auto. destruct H3; auto.
+    exfalso; apply H2; auto.
+  Qed.
+
+  Lemma NoDupSame_remove: forall a l1 l2 l1' l2', 
+    NoDupSame (l1 ++ a :: l2) (l1' ++ a :: l2') -> NoDupSame (l1 ++ l2) (l1' ++ l2').
+  Proof.
+    intros. inv H. eapply NoDupSame_intro.
+    - eapply NoDup_remove_1; eauto.
+    - eapply NoDup_remove_1; eauto.
+    - intro; intros.
+      assert(a0 <> a). eapply NoDup_remove in H0 as [].
+      intro; subst. apply H4; auto.
+      assert(In a0 (l1' ++ a :: l2')). eapply H2.
+      apply in_app_or in H. destruct H. apply in_or_app; left; auto.
+      apply in_or_app; right; right; auto. eapply in_or_app.
+      eapply in_app_or in H5; destruct H5. left; auto. right. destruct H5; auto.
+      subst; exfalso; auto.
+    - intro; intros.
+      assert(a0 <> a). eapply NoDup_remove in H1 as [].
+      intro; subst. apply H4; auto.
+      assert(In a0 (l1 ++ a :: l2)). eapply H3.
+      apply in_app_or in H. destruct H. apply in_or_app; left; auto.
+      apply in_or_app; right; right; auto. eapply in_or_app.
+      eapply in_app_or in H5; destruct H5. left; auto. right. destruct H5; auto.
+      subst; exfalso; auto.
+  Qed.
+
+  Lemma ngt_in: forall x a l, ngt x l -> In a l -> ~ R a x.
+  Proof.
+    induction l; intros. exfalso; auto.
+    eapply ngt_cons_inv in H as []. destruct H0. subst; auto.
+    eapply IHl; auto.
+  Qed.
+
+  Lemma ngt_incl: forall l1 l2 a, incl l1 l2 -> ngt a l2 -> ngt a l1.
+  Proof.
+    induction l1; intros. eapply ngt_nil.
+    eapply ngt_cons. assert(incl l1 l2). intro; intros; eapply H; right; auto.
+    eapply IHl1; eauto.
+    assert(In a l2). apply H; left; auto. eapply ngt_in; eauto.
+  Qed.
+
+  Lemma NoDupSame_ngt: forall l1 l2 a, NoDupSame l1 l2 -> ngt a l1 -> ngt a l2.
+  Proof. intros. inv H. eapply ngt_incl; eauto. Qed.
+
+  Lemma sorted_same_elements_topo_reorder_ind:
+    forall n,
+    (forall k l1 l2, k < n -> length l1 = k -> NoDupSame l1 l2 ->  
+              topo_sorted l1 -> topo_sorted l2 -> topo_reorder l1 l2) ->
+    (forall l1 l2, length l1 = n -> NoDupSame l1 l2 ->  
+              topo_sorted l1 -> topo_sorted l2 -> topo_reorder l1 l2) .
+  Proof.
+    intros. destruct n.
+    - rewrite length_zero_iff_nil in H0; subst.
+      eapply NoDupSame_nil in H1; subst. eapply topo_reorder_nil.
+    - destruct l1. simpl in H0; inv H0. simpl in H0. inversion H0.
+      inversion H1 as []; subst. assert(In a l2). apply H7; left; auto.
+      eapply List.in_split in H5 as [l21 [l22]]. subst.
+      assert(topo_reorder (a::l1) (a::l21 ++ l22)).
+      { eapply topo_reorder_skip. inv H2; eauto.
+        eapply H; eauto.
+        - inv H1. assert(TMP: a :: l1 = [] ++ a :: l1); auto. 
+          rewrite TMP in H5, H7, H8. eapply NoDupSame_intro.
+          eapply (NoDup_remove_1 [] l1 a H4). eapply NoDup_remove_1; eauto.
+          eapply incl_remove in H7; eauto. eapply incl_remove in H8; eauto.
+        - eapply topo_sorted_cons_inv2; eauto.
+        - eapply topo_sorted_remove; eauto.
+      }
+      assert(topo_reorder (a::l21 ++ l22) (l21 ++ a :: l22)).
+      { assert(TMP1: l21 ++ a :: l22 = (l21 ++ [a]) ++ l22).
+        erewrite <- app_assoc; simpl; auto. rewrite TMP1.
+        assert(TMP2: a :: l21 ++ l22 = (a :: l21) ++ l22); auto. rewrite TMP2.
+        eapply topo_reorder_symmetry.  
+        eapply topo_reorder_app. rewrite <- app_assoc; auto.
+        eapply topo_reorder_tail_to_head.
+        replace (l21 ++ a :: l22) with ((l21 ++ [a]) ++ l22) in H3; auto.
+        eapply topo_sorted_split_l; eauto.
+        eapply topo_sorted_cons. replace (a :: l1) with ([] ++ [a] ++ l1) in H1; auto.
+        eapply NoDupSame_remove in H1. simpl in H1. eapply ngt_app_inv_l.
+        eapply NoDupSame_ngt; eauto. inv H2; auto.
+        eapply topo_sorted_split_l; eauto.
+        replace (a :: l1) with ([] ++ a :: l1) in H1; auto.
+        eapply NoDupSame_remove in H1 as ?. simpl in H9.
+        eapply NoDupSame_ngt in H9; eauto. eapply ngt_app_inv_l; eauto.
+        inv H2; auto.
+      }
+      eapply topo_reorder_trans; eauto.
+  Qed.
+
+  Lemma sorted_same_elements_topo_reorder':
+    forall n l1 l2, length l1 = n -> NoDupSame l1 l2 ->  
+      topo_sorted l1 -> topo_sorted l2 -> topo_reorder l1 l2.
+  Proof.
+    intros n. eapply sorted_same_elements_topo_reorder_ind; eauto.
+    induction n.
+    - intros. inv H.
+    - intros. assert(k < n \/ k = n). inv H; auto.
+      destruct H4.
+      eapply IHn; eauto. subst.
+      eapply sorted_same_elements_topo_reorder_ind; eauto.
+  Qed.
+
+
+  Theorem sorted_same_elements_topo_reorder: 
+    forall l1 l2,  NoDupSame l1 l2 -> 
+      topo_sorted l1 -> topo_sorted l2 -> topo_reorder l1 l2.
+  Proof.
+    intros. eapply sorted_same_elements_topo_reorder'; eauto.
+  Qed.
+
+
+End TOPO_REORDER.
+
+
+
+
+
+
+Open Scope positive_scope.
+Require Import Lia.
+
+Section LIST_TOPO.
+
+  Context {A: Type}.
+
+  Fixpoint numlistgen' (l: list A) (n: positive): list (positive * A) :=
+    match l with
+    | [] => []
+    | x :: l' => (n, x) :: numlistgen' l' (n + 1)
+    end.
+  
+  Check numlistgen'.
+
+  Definition numlistgen (l: list A) := numlistgen' l 1.
+
+  Fixpoint numlistoff (l: list (positive * A)): list A :=
+    match l with
+    | [] => []
+    | (n, x) :: l' => x :: numlistoff l'
+    end.
+
+  Lemma numlistgen_length': forall l i, length l = length (numlistgen' l i).
+  Proof. induction l; intros. simpl; auto. simpl. erewrite <- IHl; auto. Qed.
+
+  Lemma numlistgen_length: forall l, length l = length (numlistgen l).
+  Proof. intros. eapply numlistgen_length'. Qed.
+
+  Lemma numlist_gen_off0: forall l i, numlistoff (numlistgen' l i) = l.
+  Proof. induction l; simpl; auto; intros. erewrite IHl; auto. Qed.
+  
+  Lemma numlist_gen_off: forall l, numlistoff (numlistgen l) = l.
+  Proof. intros. apply numlist_gen_off0. Qed.
+  
+
+  Definition NoDupNum (l: list (positive * A)) := NoDup (List.map fst l).
+
+  Lemma NoDupNum_cons_inv: forall nl na, NoDupNum (na :: nl) -> NoDupNum nl.
+  Proof.
+    induction nl; simpl; intros. apply NoDup_nil.
+    unfold NoDupNum in *. simpl in *. eapply NoDup_cons.
+    inv H; inv H3; auto.
+    eapply IHnl. eapply NoDup_cons. inv H; inv H3; eauto.
+    inv H; inv H3; eauto.
+  Qed.
+
+  Lemma numblistgen_low_bound: forall l i j a,
+    In (j, a) (numlistgen' l i) -> i <= j.
+  Proof.
+    induction l; intros. 
+    - simpl in H. exfalso; auto.
+    - simpl in H. destruct H.
+      + inv H. lia.
+      + specialize (IHl _ _ _ H). lia.
+  Qed.
+
+  Lemma numbered_list_nodup_number0: forall l i, NoDupNum (numlistgen' l i).
+  Proof.
+    assert(TMP: forall (nl: list (positive * A)) i, In i (List.map fst nl) -> exists a, In (i, a) nl).
+    { induction nl; simpl; intros.
+      - exfalso; auto.
+      - destruct a as [pos a]. simpl in H. destruct H.
+        subst. exists a; auto.
+        eapply IHnl in H as []. exists x; auto. }
+    induction l.
+    - intros. simpl. apply NoDup_nil.
+    - intros. simpl. unfold NoDupNum. simpl. apply NoDup_cons.
+      intro. eapply TMP in H as [].
+      eapply numblistgen_low_bound in H. lia.
+      apply IHl.
+  Qed.
+
+  Lemma numlistgen_NoDupNum: forall l, NoDupNum (numlistgen l).
+  Proof. intros. apply numbered_list_nodup_number0. Qed.
+
+  Lemma nodup_number_nodup: forall l, NoDupNum l -> NoDup l.
+  Proof.
+    induction l. intros.
+    - apply NoDup_nil.
+    - intros. apply NoDup_cons. inv H.
+      intro. apply H2.
+      assert(TMP: forall l x, In x l -> In (fst x) (map (fun p : positive * A => fst p) l)).
+      { induction l0; intros; auto. destruct H0. subst. left; auto.
+        right. eapply IHl0; auto. }
+      apply TMP; auto.
+      apply IHl. apply NoDup_cons_iff in H as []; auto.
+  Qed.
+
+  Lemma numlistgen_NoDup: forall l, NoDup (numlistgen l).
+  Proof. intros. apply nodup_number_nodup, numlistgen_NoDupNum. Qed.
+
+  Lemma numlist_in_num_in: forall (nl: list (positive * A)) x, In x nl -> In (fst x) (map fst nl).
+  Proof.
+    induction nl. intros; simpl; auto.
+    intros. simpl. destruct H; subst; auto.
+  Qed.
+
+  Lemma numlist_incl_num_incl: forall nl nl': list (positive*A), 
+    incl nl nl' -> incl (map fst nl) (map fst nl').
+  Proof.
+    induction nl. intros; simpl. eapply incl_nil_l.
+    intros. eapply incl_cons_inv in H as []. simpl. eapply incl_cons.
+    eapply numlist_in_num_in; eauto. eapply IHnl; eauto.
+  Qed.
+
+
+  Lemma topo_reorder_NoDupNum_preserved:
+    forall R nl nl', topo_reorder R nl nl' -> NoDupNum nl' -> NoDupNum nl.
+  Proof.
+    assert(TMP: forall l x, In x l -> In (fst x) (map (fun p : positive * A => fst p) l)).
+    { induction l; intros; auto. destruct H. subst. left; auto.
+      right. eapply IHl; auto. }
+    intros. induction H.
+    - eapply NoDup_nil.
+    - unfold NoDupNum in *. simpl in *.
+      inv H0. eapply NoDup_cons; eauto.
+      intro; apply H4. 
+      eapply topo_reorder_incl in H1; eauto. eapply numlist_incl_num_incl in H1.
+      eapply H1; auto.
+    - unfold NoDupNum in *. simpl in *. inv H0; subst; auto.
+      inv H5; subst; auto. eapply NoDup_cons.
+      intro. destruct H0. apply H4; rewrite H0; left; auto. apply H3; auto.
+      eapply NoDup_cons; auto. intro. apply H4; right; auto.
+    - eapply IHtopo_reorder1, IHtopo_reorder2; auto.
+  Qed.
+
+  Variable R: A -> A -> Prop.
+  Variable l: list A.
+
+  (* Generated Relation from a list *)
+  (* Inductive GenR (na1 na2: positive * A): Prop :=
+   GenR_intro: List.In na1 (numlistgen l) -> List.In na2 (numlistgen l) -> 
+    fst na1 < fst na2 -> R (snd na1) (snd na2)  -> GenR na1 na2
+  . *)
+
+  (* Generated Relation from a list,
+      aux. definition for simpler proofs *)
+  Inductive GenR' (i: positive) (na1 na2: positive * A): Prop :=
+    GenR_intro: List.In na1 (numlistgen' l i) -> List.In na2 (numlistgen' l i) -> 
+    fst na1 < fst na2 -> R (snd na1) (snd na2)  -> GenR' i na1 na2
+  .
+
+  (* Generated Relation from a list *)
+  Definition GenR := GenR' 1.
+  
+  Definition treorder' := fun i => topo_reorder (GenR' i).
+  Definition tsorted' := fun i => topo_sorted (GenR' i).
+
+  Definition treorder := topo_reorder GenR.
+  Definition tsorted := topo_sorted GenR.
+
+  Lemma treorder_self': forall i j, treorder' i (numlistgen' l j) (numlistgen' l j).
+  Proof.
+    induction l; intros; simpl. apply topo_reorder_nil.
+    eapply topo_reorder_skip.
+    - eapply ngt'_ngt. intro; intros. destruct x.
+      eapply numblistgen_low_bound in H. intro. inv H0. simpl in H3. lia.
+    - eapply IHl0.
+  Qed. 
+
+  Lemma treorder_self: treorder (numlistgen l) (numlistgen l).
+  Proof. apply treorder_self'. Qed.
+
+  Lemma tsorted_self': forall i j, tsorted' i (numlistgen' l j).
+  Proof.
+    induction l; intros; simpl. eapply topo_sorted_nil.
+    eapply topo_sorted_cons.
+    - eapply ngt'_ngt. intro. intros. destruct x.
+      eapply numblistgen_low_bound in H. intro. inv H0. simpl in H3. lia.
+    - eapply IHl0.
+  Qed.
+
+  Lemma tsorted_self: tsorted (numlistgen l).
+  Proof. eapply tsorted_self'. Qed.
+
+End LIST_TOPO.
+
+
+Section SWAPPING_PROPERTY.
+  Context {A: Type}.
+  Variable Rb: A -> A -> bool.
+  Hypothesis SymmetricR: forall x y, Rb x y = Rb y x.
+
+  Let Rbnum (na1 na2: positive * A) := Rb (snd na1) (snd na2).
+  Let R := fun x y => Rb x y = true.
+
+  Lemma SymmetricRbnum: forall x y, Rbnum x y = Rbnum x y.
+  Proof. destruct x; destruct y. unfold Rbnum; simpl. rewrite SymmetricR; auto. Qed.
+
+  Theorem swapping_property_general:
+    forall l nl1 nl2, List.incl nl1 (numlistgen l) ->
+      (* List.incl nl2 (numlistgen l) ->  *)
+      (treorder R l) nl1 nl2 -> 
+      NoDupNum nl1 ->
+        exists ln, nl2 = try_swap_seq Rbnum ln nl1.
+  Proof.
+    intros. induction H0. 
+    - exists []. simpl. auto.
+    - eapply List.incl_cons_inv in H as [].
+      unfold NoDupNum in H1. eapply NoDupNum_cons_inv in H1.
+      eapply IHtopo_reorder in H3 as [ln]; eauto.
+      exists (List.map Datatypes.S ln).
+      assert(TMP: forall lnx lx, try_swap_seq Rbnum (map Datatypes.S lnx) (x :: lx) 
+                = x :: try_swap_seq Rbnum lnx lx).
+      { induction lnx. simpl; intros; auto.
+        intros. simpl. destruct lx.
+        + rewrite try_swap_nil. erewrite try_swap_seq_singleton.
+          erewrite try_swap_seq_nil. auto.
+        + erewrite IHlnx; auto. }
+      rewrite TMP, H3; auto.
+    - exists [O]. simpl.
+      assert(Rbnum y x = false). 2:{ rewrite H3; auto. }
+      remember (Rbnum y x) as b. destruct b; auto.
+      exfalso. symmetry in Heqb.
+      destruct (Pos.lt_total (fst x) (fst y)).
+      { apply H0. apply GenR_intro; auto.
+        eapply List.incl_cons_inv in H as []; eauto.
+        eapply List.incl_cons_inv in H4 as []; eauto.
+        eapply List.incl_cons_inv in H as []; eauto.
+        unfold R. rewrite SymmetricR; auto. } destruct H3.
+      { inv H1. apply H6. subst; left; auto. }
+      { apply H2. apply GenR_intro; auto.
+        eapply List.incl_cons_inv in H as[]; eauto.
+        eapply List.incl_cons_inv in H as[]; eauto.
+        eapply List.incl_cons_inv in H4 as[]; eauto. }
+     - assert(NoDupNum l'). eapply topo_reorder_symmetry in H0_.
+       eapply topo_reorder_NoDupNum_preserved in H0_; eauto.
+       assert(incl l' (numlistgen l)). eapply topo_reorder_symmetry in H0_.
+       pose proof (treorder_self R l); unfold treorder in H2.
+       eapply topo_reorder_incl in H0_; eauto. eapply incl_tran; eauto. 
+       edestruct IHtopo_reorder1 as [ln1]; eauto. edestruct IHtopo_reorder2 as [ln2]; eauto.
+       exists (ln1 ++ ln2).
+       subst. erewrite try_swap_app; auto.
+  Qed.
+
+  Theorem swapping_property:
+    forall l nl', (treorder R l) (numlistgen l) nl' -> 
+      exists ln, nl' = try_swap_seq Rbnum ln (numlistgen l).
+  Proof.
+    intros. eapply swapping_property_general; eauto. apply List.incl_refl.
+    eapply numlistgen_NoDupNum.
+  Qed.
+
+End SWAPPING_PROPERTY.
+
+
+Section TRY_SWAP_NUM.
+  Open Scope nat_scope.
+  Context {A: Type}.
+  Variable (rel: A -> A -> bool).
+
+  Let rel_num (na1 na2: positive * A) := rel (snd na1) (snd na2).
+
+  Lemma num_list_equal_content_equal_swap:
+    forall nl l n, l = numlistoff nl ->
+      numlistoff (try_swap rel_num n nl) = try_swap rel n l.
+  Proof.
+    induction nl.
+    - simpl; intros. subst. erewrite! try_swap_nil. auto.
+    - intros. destruct a. simpl in H.
+      destruct nl.
+      { simpl in H. subst. rewrite! try_swap_singleton. simpl; auto. }
+      { destruct n.
+        + destruct p0. simpl in H. subst. simpl.
+          unfold rel_num; simpl. destruct (rel a a0); simpl; auto.
+        + subst. destruct p0. simpl. erewrite IHnl; eauto. }
+  Qed.
+
+  Lemma num_list_equal_content_equal_swap_seq:
+    forall ln l nl, l = numlistoff nl ->
+      numlistoff (try_swap_seq rel_num ln nl) = try_swap_seq rel ln l.
+  Proof.
+    induction ln; intros.
+    - simpl; auto.
+    - simpl. erewrite IHln; eauto.
+      erewrite num_list_equal_content_equal_swap; eauto.
+  Qed.
+
+  Lemma try_swap_seq_num_equally: forall ln l,
+    numlistoff (try_swap_seq rel_num ln (numlistgen l)) = try_swap_seq rel ln l.
+  Proof.
+    intros; apply num_list_equal_content_equal_swap_seq.
+    erewrite numlist_gen_off; eauto.
+  Qed.
+
+End TRY_SWAP_NUM.
+
+
+Require Import Errors.
+Require Import AST Integers Values Events Memory Linking Globalenvs Smallstep.
+Require Import Op Locations Conventions Machregs LTL.
+Require Import Linear Asmgenproof0 Asmgenproof.
+
+
+Open Scope error_monad_scope.
+Import ListNotations.
+Open Scope list_scope.
+
+Section SIMULATION_SEQUENCE.
+  Variable F V: Type.
+
+  Definition transf_program_one (transf_def: ident -> fundef -> fundef) :=
+      transform_partial_program2
+        (fun i f => OK (transf_def i f)) 
+        (fun i (v:unit) => OK v).
+
+  Fixpoint transf_program_sequence (tfl: list (ident -> fundef -> fundef)) (p: program) := 
+    match tfl with
+    | nil => OK p
+    | transf_fundef :: tfl' => 
+        do p' <- transf_program_one transf_fundef p;
+        transf_program_sequence tfl' p'
+    end.
+
+  Definition transf_single_fun_fsim_preserve (transf_def: ident -> fundef -> fundef):=
+    forall prog tprog, 
+    transform_partial_program2 
+      (fun i f => OK (transf_def i f)) (fun i v => OK v) prog = OK tprog ->
+    forward_simulation (Linear.semantics prog) 
+    (Linear.semantics tprog).
+
+  Definition transf_fundef_list_preserved(lf: list (ident -> fundef -> fundef)): Prop :=
+    Forall transf_single_fun_fsim_preserve lf.
+
+  Variable prog: program.
+  Variable tprog: program.
+  Variable tfl: list (ident -> fundef -> fundef).
+  Hypothesis safe_list: transf_fundef_list_preserved tfl.
+  Hypothesis TRANSF_PROG: transf_program_sequence tfl prog = OK tprog.
+  
+  Theorem forward_simulation_sequence:
+    forward_simulation (Linear.semantics prog) 
+                       (Linear.semantics tprog).
+  Proof.
+    revert prog tprog TRANSF_PROG.
+    induction safe_list; intros.
+    - inv TRANSF_PROG. apply forward_simulation_refl.
+    - inv safe_list. specialize (IHt H3).
+      simpl in TRANSF_PROG. monadInv TRANSF_PROG. rename x0 into tmprog.
+      eapply compose_forward_simulations 
+        with (L2:= semantics tmprog); auto.
+  Qed.
+
+  (* Definition real_match_prog (prog tprog: program) :=
+    match_program (fun ctx f tf => real_transf_fundef f = OK tf) eq prog tprog. *)
+
+End SIMULATION_SEQUENCE.
+
+
+(* TODO Warning: simple but machine dependent;
+      Try to make codes the same *)
+
+Section MACHINE_DEPENDENT_RISCV.
+
+Lemma eval_op_genv_irrelevent: forall prog tprog: program,
+  let ge := Genv.globalenv prog in
+  let tge := Genv.globalenv tprog in
+    forall sp op lv m 
+    (SYMB: forall s, Genv.find_symbol tge s = Genv.find_symbol ge s),
+      eval_operation ge sp op lv m = eval_operation tge sp op lv m.
+Proof.
+  intros. destruct lv; auto. destruct op; simpl; auto.
+  unfold Genv.symbol_address. rewrite SYMB; auto.
+Qed.
+
+Lemma eval_addr_genv_irrelevent: forall prog tprog: program,
+let ge := Genv.globalenv prog in
+let tge := Genv.globalenv tprog in
+  forall sp addr lv
+  (SYMB: forall s, Genv.find_symbol tge s = Genv.find_symbol ge s),
+  eval_addressing ge sp addr lv = eval_addressing tge sp addr lv.
+Proof.
+  intros. destruct lv; auto. destruct addr; simpl; auto.
+  unfold Genv.symbol_address. rewrite SYMB; auto.
+Qed.
+
+Definition mem_read_op (op: operation) :=
+  match op with
+  | Ocmp _   => true
+  (* | Osel _ _ => true   *)
+      (* riscv does not have this op; compatible for x86, arm, powerpc, aarch64 *)
+  | _ => false
+  end.
+
+Lemma eval_op_mem_irrelevant: forall prog: program,
+let ge := Genv.globalenv prog in
+  forall op sp rs m1 m2, mem_read_op op = false ->
+    eval_operation ge sp op rs m1 = eval_operation ge sp op rs m2.
+Proof. intros. destruct op; auto; simpl in H; discriminate H. Qed. 
+
+End MACHINE_DEPENDENT_RISCV.
+
+(* Section MACHINE_DEPENDENT_X86.
+
+  Lemma eval_op_genv_irrelevent: forall prog tprog: program,
+    let ge := Genv.globalenv prog in
+    let tge := Genv.globalenv tprog in
+      forall sp op lv m 
+      (SYMB: forall s, Genv.find_symbol tge s = Genv.find_symbol ge s),
+        eval_operation ge sp op lv m = eval_operation tge sp op lv m.
+  Proof.
+    intros. destruct lv; auto. destruct op; simpl; auto.
+    unfold Genv.symbol_address. rewrite SYMB; auto.
+    unfold eval_addressing64. destruct Archi.ptr64; auto.
+    destruct a; auto. unfold Genv.symbol_address. rewrite SYMB; auto.
+  Qed.
+
+  Lemma eval_addr_genv_irrelevent: forall prog tprog: program,
+  let ge := Genv.globalenv prog in
+  let tge := Genv.globalenv tprog in
+    forall sp addr lv
+    (SYMB: forall s, Genv.find_symbol tge s = Genv.find_symbol ge s),
+    eval_addressing ge sp addr lv = eval_addressing tge sp addr lv.
+  Proof.
+    intros. destruct lv; auto. destruct addr; simpl; auto.
+    unfold eval_addressing. unfold eval_addressing64. destruct Archi.ptr64; auto. 
+    unfold Genv.symbol_address. rewrite SYMB; auto.
+  Qed.
+
+  Definition mem_read_op (op: operation) :=
+    match op with
+    | Ocmp _   => true
+    | Osel _ _ => true  (* riscv does not have this op; compatible for x86, arm, powerpc, aarch64 *)
+    | _ => false
+    end.
+
+  Lemma eval_op_mem_irrelevant: forall prog: program,
+  let ge := Genv.globalenv prog in
+    forall op sp rs m1 m2, mem_read_op op = false ->
+      eval_operation ge sp op rs m1 = eval_operation ge sp op rs m2.
+  Proof. intros. destruct op; auto; simpl in H; discriminate H. Qed. 
+
+End MACHINE_DEPENDENT_X86. *)
+
+Definition slot_eqb: slot -> slot -> bool.
+Proof. boolean_equality. Defined.
+
+(* Definition Z_eqb: Z -> Z -> bool.
+Proof. boolean_equality; apply (Pos.eqb p p0). Defined. *)
+
+Definition typ_eqb: typ -> typ -> bool.
+Proof. boolean_equality; apply (Pos.eqb p p0). Defined.
+
+(* Definition operation_eqb: operation -> operation -> bool.
+Proof. boolean_equality. *)
+
+Definition mreg_eqb: mreg -> mreg -> bool.
+Proof. boolean_equality. Defined.
+
+Fixpoint mreg_list_eqb (l1 l2: list mreg): bool :=
+  match l1, l2 with
+  | m1 :: l1', m2 :: l2' => mreg_eq m1 m2 && mreg_list_eqb l1' l2'
+  | nil, nil => true
+  | _, _ => false
+  end. 
+
+Definition chunk_eqb: memory_chunk -> memory_chunk -> bool.
+Proof. boolean_equality. Defined.
+
+
+Lemma mreg_ident_eq: forall (s1 s2: mreg + ident), {s1 = s2} + {s1 <> s2}.
+Proof. generalize mreg_eq ident_eq. decide equality. Defined.
+
+(* Definition instruction_eqb: instruction -> instruction -> bool.
+Proof. 
+  generalize mreg_eq typ_eq slot_eq Z.eq_dec eq_addressing eq_operation chunk_eq signature_eq
+    mreg_ident_eq external_function_eq eq_condition peq.
+  boolean_equality. admit. admit.
+Admitted. *)
+
+
+Lemma mreg_eqb_refl: forall x, mreg_eqb x x = true.
+Proof. intros. destruct x; simpl; auto. Qed.
+
+Lemma mreg_eqb_eq: forall x y, mreg_eqb x y = true -> x = y.
+Proof. BE.bool_eq_sound. Qed.
+
+Lemma mreg_eqb_eq_iff: forall x y, mreg_eqb x y = true <-> x = y.
+Proof. split. apply mreg_eqb_eq. intros; subst. apply mreg_eqb_refl. Qed.
+
+
+(** [i1: reg = ...] :: [i2: ... = op args] :: [...] *)
+Fixpoint mreg_in_list (reg: mreg) (regs: list mreg): bool :=
+  match regs with
+  | nil => false
+  | reg' :: regs' => mreg_eq reg reg' || mreg_in_list reg regs'
+  end.
+
+Fixpoint mreg_list_intersec (regs1 regs2: list mreg): bool :=
+  match regs1 with
+  | nil => false
+  | reg1 :: regs1' => mreg_in_list reg1 regs2 || mreg_list_intersec regs1' regs2  
+  end.
+
+(* instructions that cannot be re-ordered *)
+Definition solid_inst (i: instruction): bool :=
+  match i with
+  | Lcall _ _  | Ltailcall _ _  | Lbuiltin _ _ _ 
+  | Llabel _  | Lgoto _ | Lcond _ _ _ | Ljumptable _ _
+  | Lreturn 
+  | Lgetstack _ _ _ _ | Lsetstack _ _ _ _
+      => true
+  | _ => false
+  end.
+
+(* Some true: memory write, Some false: memory read. None: no memory operation *)
+(* Note: when linear was transformed to Mach, set/get stack inst. will access memory,
+    though it is seperate *)
+Definition mem_write (i: instruction): option bool :=
+  match i with
+  | Lgetstack _ _ _ _ => Some false
+  | Lsetstack _ _ _ _ => Some false
+  | Lop op _ _ => if mem_read_op op then Some false else None
+  | Lload _ _ _ dst => Some false
+  | Lstore _ _ _ src => Some true
+  | _ => None
+  end. 
+
+Definition get_dst (i: instruction): option mreg :=
+  match i with
+  | Lgetstack _ _ _ dst
+  | Lop _ _ dst | Lload _ _ _ dst => Some dst
+  | _ => None
+  end. 
+
+Definition get_srcs (i: instruction): list mreg :=
+  match i with
+  | Lop op args res => args
+  | Lload _ _ args _ => args
+  | Lsetstack src _ _ _   => src :: nil
+  | Lstore _ _ args src => src::args
+  | _ => nil
+  end.
+
+Definition destroyed_by (i: instruction):=
+  match i with
+  | Lgetstack sl _ _ _ =>     destroyed_by_getstack sl
+  | Lsetstack _ _ _ ty =>     destroyed_by_setstack ty
+  | Lop op _ _ =>             destroyed_by_op op
+  | Lload chunk addr _ _ =>   destroyed_by_load chunk addr
+  | Lstore chunk addr _ _ =>  destroyed_by_store chunk addr
+  | Lbuiltin ef _ _ =>        destroyed_by_builtin ef
+  | Lcond cond _ _ =>         destroyed_by_cond cond
+  | Ljumptable _ _ =>         destroyed_by_jumptable
+  | _ => nil 
+  end.
+
+(* RAW/True-dependence: i1 write register r, then i2 read from [..., r, ...]  *)
+Definition hb_wr (i1 i2: instruction):=
+    match get_dst i1, get_srcs i2 with 
+    | Some dst, srcs  => mreg_in_list dst srcs
+    | _, _ => false
+    end.
+
+(* WAR/Anti-dependence: i1 read from [..., r, ...], then i2 write register r,  *)
+Definition hb_rw (i1 i2: instruction) :=
+  hb_wr i2 i1.
+
+(* WAW/Output-dependence: i1 write register r, then i2 write register r*)
+Definition hb_ww (i1 i2: instruction) :=
+    match get_dst i1, get_dst i2 with 
+    | Some dst1, Some dst2 =>
+        if mreg_eq dst1 dst2 then true else false
+    | _, _ => false
+    end.
+
+(* Mem dependence: one of i1 and i2 write to memory, another also read/write memory *)
+(* always a dependence since no alias analysis performed *)
+Definition hb_mem (i1 i2: instruction):=
+    match mem_write i1, mem_write i2 with
+    | Some true, Some _ | Some _, Some true => true 
+    | _, _ => false
+    end.
+
+Definition hb_destroy_src (i1 i2: instruction) :=
+  mreg_list_intersec (get_srcs i1) (destroyed_by i2).
+  
+Definition hb_destroy_dst (i1 i2: instruction) :=
+  match get_dst i1 with
+  | Some dst => mreg_in_list dst (destroyed_by i2)
+  | None => false
+  end.
+
+Definition hb_destroy (i1 i2: instruction) :=
+  hb_destroy_src i1 i2
+  || hb_destroy_src i2 i1
+  || hb_destroy_dst i1 i2
+  || hb_destroy_dst i2 i1.
+
+(* Dependence relation:
+    i1 i2 should always happens before i2 if it happens before in original code
+      note this relation is order irrelevent thus symmetric *)
+Definition happens_before (i1 i2: instruction): bool :=
+    (* solid dependence from control inst. like function calls, return, etc. *)
+    solid_inst i1
+    || solid_inst i2
+    (* register dependence *)
+    || hb_rw i1 i2 || hb_rw i2 i1 || hb_ww i1 i2
+    (* memory dependence without alias information 
+        - any two memory access with at least write are regarded to have dependence *)
+    || hb_mem i1 i2
+    (* destroyed registers during each step *)
+    || hb_destroy i1 i2.
+
+Notation "i1 D~> i2":= (happens_before i1 i2) (at level 1).
+
+Definition try_swap_code:= try_swap happens_before.
+
+Definition try_swap_nth_func (n: nat)(f: function):= 
+    mkfunction f.(fn_sig) f.(fn_stacksize) (try_swap_code n f.(fn_code)) .
+
+Lemma happens_before_symmetric: 
+  forall i1 i2, happens_before i1 i2 = happens_before i2 i1.
+Proof.
+  intros. unfold happens_before in *. remember (solid_inst i1) as b. destruct b.
+Admitted. 
+
+Lemma solid_inst_indep1: forall i1 i2, solid_inst i1 = true -> i1 D~> i2 = true.
+Proof. intros. destruct i1, i2; simpl in *; try discriminate H; auto. Qed.
+
+Lemma indep_inv_not_solid1: forall i1 i2, i1 D~> i2 = false -> solid_inst i1 = false.
+Proof. intros. remember (solid_inst i1) as b. destruct b. symmetry in Heqb. 
+  unfold happens_before in H. rewrite Heqb in H; auto. auto. Qed.
+
+Lemma indep_inv_not_solid2: forall i1 i2, i1 D~> i2 = false -> solid_inst i2 = false.
+Proof. intros. remember (solid_inst i2) as b2. symmetry in Heqb2. unfold happens_before in H. 
+    destruct b2; rewrite Heqb2 in H; destruct (solid_inst i1); auto. Qed.
+
+
+Section LOCSET_AGREE.
+
+  Definition lsagree (rs rs': locset) := 
+    forall r: loc, Locmap.get r rs = Locmap.get r rs'.
+
+  Lemma lsagree_refl: reflexive _ lsagree.
+  Proof. hnf; intros; intro; auto. Qed.
+
+  Lemma lsagree_symmetric: symmetric _ lsagree.
+  Proof. hnf; intros; intro; auto. Qed.
+
+
+  Lemma lsagree_get: forall rs rs' r, lsagree rs rs' -> rs r = rs' r.
+  Proof. intros. apply H. Qed.
+
+  Lemma lsagree_getpair: 
+    forall rs rs' pr, lsagree rs rs' -> Locmap.getpair pr rs = Locmap.getpair pr rs'.
+  Proof. 
+    intros. destruct pr; simpl. apply H. 
+    hnf in H; unfold Locmap.get in H. repeat rewrite H; auto.
+  Qed.
+
+  Lemma lsagree_undef_caller_save_regs: forall rs rs', lsagree rs rs' -> 
+    lsagree (LTL.undef_caller_save_regs rs) (LTL.undef_caller_save_regs rs').
+  Proof. 
+    intros; intro. unfold Locmap.get, LTL.undef_caller_save_regs.
+    destruct r. destruct (is_callee_save r); auto. apply H. destruct sl; auto; eapply H.
+  Qed. 
+
+  Lemma lsagree_set:
+    forall p v rs rs', lsagree rs rs' ->
+      lsagree (Locmap.set p v rs) (Locmap.set p v rs').
+  Proof. intros; intro. unfold Locmap.get, Locmap.set. destruct (Loc.eq p r); auto.
+    destruct (Loc.diff_dec p r); auto. apply H. Qed.
+
+  Lemma lsagree_setpair:
+    forall p v rs rs', lsagree rs rs' ->
+      lsagree (Locmap.setpair p v rs) (Locmap.setpair p v rs').
+  Proof. 
+    intros; intro. unfold Locmap.get, Locmap.setpair. 
+    destruct p; auto; unfold Locmap.set; auto.
+    - destruct (Loc.eq (R r0) r); auto. destruct (Loc.diff_dec (R r0) r); auto. apply H.
+    - destruct (Loc.eq (R rlo) r); auto. destruct (Loc.diff_dec (R rlo) r); auto.
+    destruct (Loc.eq (R rhi) r); auto. destruct (Loc.diff_dec (R rhi) r); auto. apply H.
+  Qed.
+
+  Lemma lsagree_reglist: forall rs rs' rl, 
+    lsagree rs rs' -> LTL.reglist rs rl = LTL.reglist rs' rl.
+  Proof. intros. induction rl; auto. simpl. rewrite IHrl. erewrite lsagree_get; eauto. Qed. 
+
+  Lemma lsagree_call_regs: forall rs rs',
+    lsagree rs rs' -> lsagree (LTL.call_regs rs) (LTL.call_regs rs').
+  Proof. 
+    intros. intro. destruct r; unfold Locmap.get, LTL.call_regs; simpl.
+    - eapply H. - destruct sl; auto. eapply H. 
+  Qed.
+
+  Lemma lsagree_undef_regs: forall rs rs' rl,
+    lsagree rs rs' -> lsagree (LTL.undef_regs rl rs) (LTL.undef_regs rl rs').
+  Proof.
+    intros; intro. induction rl; auto. simpl.
+    unfold Locmap.get, Locmap.set. destruct (Loc.eq (R a) r); auto.
+    destruct (Loc.diff_dec (R a) r); auto.
+  Qed.
+
+  Lemma lsagree_return_regs: forall rsa rsb rsa' rsb',
+    lsagree rsa rsa' -> lsagree rsb rsb' ->
+      lsagree (LTL.return_regs rsa rsb) (LTL.return_regs rsa' rsb').
+  Proof. intros. intro. unfold Locmap.get, LTL.return_regs. destruct r; auto.
+    destruct (is_callee_save r); eapply lsagree_get; auto.
+    destruct sl; auto; eapply lsagree_get; auto. Qed.
+
+  Lemma lsagree_eval_builtin_arg:
+    forall ge rs rs' sp m arg var,
+    lsagree rs rs' -> eval_builtin_arg ge rs sp m arg var -> 
+      eval_builtin_arg ge rs' sp m arg var.
+  Proof. 
+    intros. unfold lsagree, Locmap.get in H. induction H0; try rewrite H.
+    - apply eval_BA. - apply eval_BA_int. - apply eval_BA_long.
+    - apply eval_BA_float. - apply eval_BA_single.
+    - apply eval_BA_loadstack; auto. - apply eval_BA_addrstack.
+    - apply eval_BA_loadglobal; auto. - apply eval_BA_addrglobal.
+    - apply eval_BA_splitlong; auto. - apply eval_BA_addptr; auto.
+  Qed.
+
+  Lemma lsagree_eval_builtin_args:
+    forall ge rs rs' sp m args vargs,
+    lsagree rs rs' -> eval_builtin_args ge rs sp m args vargs -> 
+      eval_builtin_args ge rs' sp m args vargs.
+  Proof. 
+    intros. hnf in *. Check list_forall2_imply.
+    eapply list_forall2_imply. eapply H0. intros; auto. 
+    eapply lsagree_eval_builtin_arg; eauto.
+  Qed.
+
+  Lemma lsagree_setres: forall res vres rs rs', lsagree rs rs' -> 
+    lsagree (Locmap.setres res vres rs) (Locmap.setres res vres rs').
+  Proof. intros res. induction res; simpl; auto.
+    intros; intro. eapply lsagree_set; auto. Qed.
+  
+  Print Locmap.set. Check Locmap.set. Check Loc.diff.
+  Locate undef_regs.
+
+  Lemma lsagree_find_function: forall ge ros rs rs', lsagree rs rs' ->
+    find_function ge ros rs = find_function ge ros rs'.
+  Proof. intros. destruct ros; simpl; auto. erewrite lsagree_get; auto. Qed.
+
+End LOCSET_AGREE.
+
+
+(* Lemma find_function_ptr_genv_irrelevent:
+  forall ge1 ge2 ros rs,
+    (forall (s: ident), Genv.find_symbol ge1 s = Genv.find_symbol ge2 s) ->
+      find_function_ptr ge1 ros rs = find_function_ptr ge2 ros rs.
+Proof. intros. destruct ros; auto; simpl. apply H. Qed. *)
+
+Lemma extcall_genv_irrelevent:
+  forall ge1 ge2 ef args m1 t res m2,
+  Senv.equiv ge1 ge2 -> 
+    external_call ef ge1 args m1 t res m2 ->
+    external_call ef ge2 args m1 t res m2.
+Proof. 
+  intros. destruct ef; simpl in *; eauto.
+  - eapply external_functions_properties; eauto.
+  (* - eapply external_functions_properties. unfold external_functions_sem. hnf in *)
+  - eapply builtin_or_external_sem_ok; eauto. - eapply builtin_or_external_sem_ok; eauto.
+  - eapply volatile_load_ok; eauto. - eapply volatile_store_ok; eauto.
+  - eapply extcall_malloc_ok; eauto. - eapply extcall_free_ok; eauto.
+  - eapply extcall_memcpy_ok; eauto.
+  - eapply extcall_annot_ok; eauto. - eapply extcall_annot_val_ok; eauto.
+  - eapply inline_assembly_properties; eauto.
+  - eapply extcall_debug_ok; eauto.
+Qed.
+
+
+Section FIND_LABEL.
+
+Lemma is_label_inv: forall lbl a, is_label lbl a = true -> a =  Llabel lbl.
+Proof. 
+  intros. destruct a; simpl in H; inv H. destruct (peq lbl l). 
+  rewrite e; auto. discriminate H1. 
+Qed.
+
+Lemma find_label_try_swap:
+  forall lbl c c' n, Linear.find_label lbl c = Some c' ->
+    exists n', Linear.find_label lbl (try_swap_code n c) = Some (try_swap_code n' c').
+Proof.
+  intros lbl c. revert lbl. induction c; intros.
+  - exists O. inv H.
+  - simpl in H. remember (is_label lbl a) as b. destruct b.
+    + inv H. destruct c'; destruct n; simpl; try rewrite <- Heqb.
+      * exists O; auto. * exists O; auto.
+      * symmetry in Heqb; eapply is_label_inv in Heqb. subst.
+        unfold happens_before; simpl. destruct (peq lbl lbl). exists (length (i :: c')). 
+        unfold try_swap_code; erewrite try_swap_at_tail; auto. exfalso; auto.
+      * exists n; auto.
+    + destruct c. simpl in H; inv H.
+      destruct n; simpl; try rewrite <- Heqb.
+      * remember (a D~> i) as b. destruct b.
+        { simpl. rewrite <- Heqb. simpl in H. rewrite H. 
+          exists (length c'). unfold try_swap_code; erewrite try_swap_at_tail; auto. } 
+        { assert(is_label lbl i = false). 
+            remember (is_label lbl i) as b. destruct b; auto. symmetry in Heqb1.
+            eapply is_label_inv in Heqb1; subst.
+            unfold happens_before in Heqb0; destruct (solid_inst a); auto.  
+          simpl; simpl in H. rewrite H0 in *. rewrite <- Heqb.
+          rewrite H. exists (length c').
+          unfold try_swap_code; erewrite try_swap_at_tail; auto. }
+      * eapply IHc in H as [n']. exists n'; eauto.
+Qed.
+
+End FIND_LABEL.
+
+
+Lemma Linear_determ: forall p, determinate (Linear.semantics p).
+Proof. 
+  constructor.
+  - intros. inv H; inv H0.
+    + split. eapply match_traces_E0. intros; auto.
+    + split. eapply match_traces_E0. intros; auto.
+    + split. eapply match_traces_E0. intros; auto. rewrite H12 in H1; inv H1; auto.
+    + split. eapply match_traces_E0. intros; auto. 
+      rewrite H14 in H1; inv H1. rewrite H15 in H2; inv H2; auto.
+    + split. eapply match_traces_E0. intros; auto. 
+      rewrite H14 in H1; inv H1; auto. rewrite H15 in H2; inv H2; auto.
+    + split. eapply match_traces_E0. intros; auto. rewrite H11 in H1; inv H1; auto.
+    + split. eapply match_traces_E0. intros; auto.
+      rewrite H13 in H2; inv H2. rewrite H15 in H4; inv H4; auto.
+    + eapply eval_builtin_args_determ in H1. 2: { eapply H13. } subst.
+      split. eapply external_call_match_traces; eauto.
+      intros. subst. eapply external_call_deterministic in H2. 2:{ eapply H14. }
+      destruct H2; subst; auto.
+    + split. eapply match_traces_E0. intros; auto.
+    + split. eapply match_traces_E0. intros; auto. rewrite H10 in H1; inv H1; auto.
+    + split. eapply match_traces_E0. intros; auto. rewrite H15 in H3; inv H3; auto.
+    + rewrite H13 in H1; inv H1. 
+    + rewrite H12 in H1; inv H1.
+    + split. eapply match_traces_E0. intros; auto.
+    + split. eapply match_traces_E0. intros; auto. rewrite H13 in H1; inv H1; auto.
+      rewrite H14 in H2; inv H2; auto. rewrite H15 in H3; inv H3; auto.
+    + split. eapply match_traces_E0. intros; auto. rewrite H9 in H1; inv H1; auto.
+    + split. eapply match_traces_E0. intros; auto. rewrite H7 in H1; inv H1; auto.
+    + split. eapply external_call_match_traces; eauto.
+      intros; subst. eapply external_call_deterministic in H2. 2:{ eapply H8. }
+      destruct H2; subst; auto.
+    + split. eapply match_traces_E0. intros; auto.
+  - hnf. intros. inv H; auto.
+    eapply ec_trace_length. eapply external_call_spec. eauto.
+    eapply ec_trace_length. eapply external_call_spec. eauto.
+  - intros. inv H. inv H0. rewrite H1 in H. inv H.
+    unfold ge in H2, H3. unfold ge0 in H5, H6.
+    rewrite H5 in H2; inv H2; auto.
+    rewrite H6 in H3; inv H3; auto.
+  - intros. hnf. intros. intro. inv H. inv H0. 
+  - intros. inv H; inv H0. rewrite H1 in H4. inv H4; auto.
+Qed.
+
+
+Definition transf_function_try_swap_nth (n: nat) (f: function) : res function :=
+  OK (try_swap_nth_func n f).
+
+Definition transf_fundef_try_swap_nth (n: nat) (f: fundef) : res fundef :=  
+  AST.transf_partial_fundef (transf_function_try_swap_nth n) f.
+
+(** only swap one independent pair in one function *)
+(* Definition transf_program_try_swap_nth_in_one (funid: ident) (n: nat) (p: program): res program :=
+  transform_partial_program2 
+  (fun i f => if ident_eq i funid then transf_fundef_try_swap_nth n f else OK f) 
+  (fun i v => OK v) p. *)
+Fixpoint try_swap_prog_def_in_one (pos: nat) (n: nat)
+                  (prog_defs: list (ident * globdef fundef unit)): 
+                  list (ident * globdef fundef unit) :=
+  match pos, prog_defs with
+  | _, nil => nil
+  | Datatypes.S pos', prog_def :: prog_defs' => 
+                        prog_def :: try_swap_prog_def_in_one pos' n prog_defs'
+  | Datatypes.O, (id, Gfun (Internal f)) :: prog_defs' => 
+                        (id, Gfun (Internal (try_swap_nth_func n f))) :: prog_defs'
+  | Datatypes.O, _ => prog_defs
+  end.
+
+Fixpoint try_swap_prog_def_seq (seq: list (nat * nat))
+                  (prog_defs: list (ident * globdef fundef unit)):=
+  match seq with
+  | nil => prog_defs
+  | (pos, n) :: seq' => try_swap_prog_def_seq seq' (try_swap_prog_def_in_one pos n prog_defs)
+  end.
+
+Definition transf_program_try_swap_in_one (pos: nat) (n: nat) (p: program): res program :=
+  OK (mkprogram (try_swap_prog_def_in_one pos n p.(prog_defs)) p.(prog_public) p.(prog_main)).
+
+Definition transf_program_try_swap_seq (seq: list (nat * nat)) (p: program): res program :=
+  OK (mkprogram (try_swap_prog_def_seq seq p.(prog_defs)) p.(prog_public) p.(prog_main) ).
+
+Inductive match_fundef0: fundef -> fundef -> Prop :=
+  | match_fundef0_internal: forall n f,
+      match_fundef0 (Internal f) (Internal (try_swap_nth_func n f))
+  | match_fundef0_external: forall f, match_fundef0 (External f) (External f)
+.
+
+Inductive match_fundef (p: program): fundef -> fundef -> Prop :=
+  | match_fundef_internal: forall n f,
+      match_fundef p (Internal f) (Internal (try_swap_nth_func n f))
+  | match_fundef_external: forall f, match_fundef p (External f) (External f)
+.
+
+Definition match_varinfo: unit -> unit -> Prop := eq.
+
+Lemma match_fundef_refl: forall p f, match_fundef p f f.
+Proof. 
+  intros. destruct f.
+  - set(n:= length (fn_code f)). 
+    assert (try_swap_nth_func n f = f). {
+      unfold try_swap_nth_func.
+      assert(try_swap_code n (fn_code f) = fn_code f). eapply try_swap_at_tail.
+      rewrite H. destruct f; reflexivity.
+    }
+    exploit match_fundef_internal.
+    instantiate(2:=n). intros. erewrite H in H0. eauto.
+  - eapply match_fundef_external.
+Qed.
+
+
+
+Lemma match_globdef_refl: forall ctx def, match_globdef match_fundef match_varinfo ctx def def.
+Proof.
+  intros. destruct def.
+  - eapply match_globdef_fun. eapply linkorder_refl.
+    eapply match_fundef_refl.
+  - eapply match_globdef_var. 
+    destruct v. simpl. eapply match_globvar_intro. eapply eq_refl.
+Qed.
+
+Lemma match_fundef_funsig: forall p f tf, match_fundef p f tf -> funsig f = funsig tf.
+Proof. intros. inv H; auto. Qed.
+
+Lemma match_fundef_match_fundef0: forall p f tf, match_fundef p f tf -> match_fundef0 f tf.
+Proof. intros. inv H. eapply match_fundef0_internal. eapply match_fundef0_external. Qed.
+
+Inductive match_stackframe: stackframe -> stackframe -> Prop :=
+  | match_stackframes_intro:
+      forall n f f' sp sp' ls ls' m c c'
+      (FUNC: try_swap_nth_func n f = f') 
+      (SP: sp = sp')  
+      (LS: lsagree ls ls')
+      (CODE: try_swap_code m c = c'),
+      match_stackframe (Stackframe f sp ls c)
+                       (Stackframe f' sp' ls' c').
+
+Definition match_stack := Forall2 match_stackframe.
+
+(* Note: use eq because we do not exploit alias analysis now;
+    otherwise, two consecutive store can be swapped *)
+Definition match_mem (m m': mem) := eq m m'.
+Ltac mem_eq := apply eq_refl.
+
+Inductive match_states: state -> state -> Prop :=
+| match_regular_state: 
+    forall sl sl' n_f f f' sp sp' n_c c c' rs rs' m m'
+    (STK: match_stack sl sl')
+    (FUNC: try_swap_nth_func n_f f = f')
+    (SP: sp = sp')
+    (CODE: try_swap_code n_c c = c' )
+    (RS: lsagree rs rs') (MEM: match_mem m m'),
+    match_states (State sl f sp c rs m)
+                 (State sl' f' sp' c' rs' m')
+| match_call_state:
+    forall sl sl' fd fd' rs rs' m m'
+    (STK: match_stack sl sl')
+    (FUNC: match_fundef0 fd fd')
+    (RS: lsagree rs rs') 
+    (MEM: match_mem m m'), (** Memory are no way to be different, since we prevented such swapping *)
+    match_states (Callstate sl fd rs m)
+                 (Callstate sl' fd' rs' m')
+| match_return_state:
+    forall sl sl' rs rs' m m'
+    (STL: match_stack sl sl')
+    (RS: lsagree rs rs') 
+    (MEM: match_mem m m'),
+    match_states (Returnstate sl rs m)
+                 (Returnstate sl' rs' m').
+
+(** Correctness proof of general correctness of instruction scheduling algorithm*)
+
+(** Step 1: prove the correctness of one single swap *)
+
+Definition match_prog (prog tprog: program) :=
+  (* let transf_fun := (fun i f => if ident_eq i funid 
+                                then transf_fundef_try_swap_nth n f else OK f) in
+  let transf_var := (fun (i: ident) (v:unit) => OK v) in *)
+  match_program_gen match_fundef match_varinfo prog prog tprog.
+
+
+Lemma match_ident_globdefs_refl:
+  forall prog_defs ctx, list_forall2
+  (match_ident_globdef match_fundef match_varinfo ctx) prog_defs prog_defs.
+Proof.
+  induction prog_defs; intros.
+  - eapply list_forall2_nil.
+  - eapply list_forall2_cons. split; auto. eapply match_globdef_refl.
+    eapply IHprog_defs.
+Qed.
+
+Lemma try_swap_prog_def_nil: forall pos n, try_swap_prog_def_in_one pos n [] = [].
+Proof. induction pos; intros; simpl; auto. Qed.
+
+
+Lemma transf_program_match':
+forall prog_defs pos n ctx,
+list_forall2 (match_ident_globdef match_fundef match_varinfo ctx) 
+              prog_defs (try_swap_prog_def_in_one pos n prog_defs).
+Proof.
+  induction prog_defs; intros.
+  - rewrite try_swap_prog_def_nil. eapply list_forall2_nil.
+  - destruct pos. 
+    + destruct a. destruct g. destruct f.
+      { simpl. eapply list_forall2_cons. split; auto. 
+      eapply match_globdef_fun. eapply linkorder_refl.
+      eapply match_fundef_internal. eapply match_ident_globdefs_refl. }
+      { simpl. eapply match_ident_globdefs_refl. }
+      { simpl. eapply match_ident_globdefs_refl. }
+    + simpl. eapply list_forall2_cons. split; auto. eapply match_globdef_refl.
+      eapply IHprog_defs.
+Qed.
+
+Lemma transf_program_match:
+forall pos n prog tprog, 
+  transf_program_try_swap_in_one pos n prog = OK tprog -> 
+    match_prog prog tprog.
+Proof.
+    intros. split. unfold transf_program_try_swap_in_one in H; inv H; simpl. 
+    eapply transf_program_match'.
+    destruct prog. unfold transf_program_try_swap_in_one in H; simpl in H; inv H.
+    split; auto.
+Qed.
+
+Require Import Globalenvs.
+
+Section SINGLE_SWAP_CORRECTNESS.
+
+  Variable prog: program.
+  Variable tprog: program.
+
+  Hypothesis TRANSF: match_program_gen match_fundef match_varinfo prog prog tprog.
+
+  Let ge := Genv.globalenv prog.
+  Let tge := Genv.globalenv tprog. 
+
+  Let tPlus := Plus (semantics tprog).
+  Let tStar := Star (semantics tprog).
+
+  Lemma symbols_preserved:
+    forall (s: ident), Genv.find_symbol tge s = Genv.find_symbol ge s.
+  Proof (Genv.find_symbol_match TRANSF).
+
+  Lemma senv_preserved:
+    Senv.equiv ge tge.
+  Proof (Genv.senv_match TRANSF).
+
+  Lemma find_function_match:
+  forall ros rs f, find_function ge ros rs = Some f ->
+    exists cunit tf, find_function tge ros rs = Some tf /\ match_fundef cunit f tf.
+  Proof.
+    intros. destruct ros; simpl in H.
+    - eapply Genv.find_funct_match 
+        with (match_fundef:=match_fundef) (match_varinfo:=match_varinfo) in TRANSF
+        as [cunit [tf [? [?]]]]. eexists cunit, tf. split; simpl; eauto. auto.
+    - remember (Genv.find_symbol ge i) as fs. destruct fs. assert(TRANSF':=TRANSF).
+      eapply Genv.find_funct_ptr_match 
+      with (match_fundef:=match_fundef) (match_varinfo:=match_varinfo) in TRANSF'
+      as [cunit [tf [? [?]]]]. eexists cunit, tf. split; simpl; eauto.
+      erewrite <- symbols_preserved in Heqfs. erewrite <- Heqfs. eauto. eauto.
+      discriminate H.
+  Qed.
+
+  Lemma exec_one_inst: forall ge sl1 f1 sp1 i1 c rs1 m1 t s2,
+  step ge (State sl1 f1 sp1 (i1 :: c) rs1 m1) t s2 -> 
+  solid_inst i1 = false ->
+    (exists sl2 f2 sp2 rs2 m2, s2 = State sl2 f2 sp2 c rs2 m2).
+  Proof. intros. assert (Hstep := H); set (s2_ := s2).
+    inv H; try discriminate H0; eexists _, _, _, _, _; eapply eq_refl. Qed.
+
+  Lemma try_swap_code_singleton: forall n i, try_swap_code n [i] = [i].
+  Proof. apply try_swap_singleton. Qed.
+
+
+  (** Case 1: Regular step without swapping **)
+  Lemma regular_state_one_step_match:
+  forall stk1 stk1' fb fb' sp sp' c c' rs1 rs1' m1 m1' s2 i t
+  (s1:= State stk1 fb sp (i :: c) rs1 m1) 
+  (STEP: step ge s1 t s2)
+  (s1':= State stk1' fb' sp' (i :: c') rs1' m1') 
+  (MAT: match_states s1 s1'),
+    exists s2', step tge s1' t s2' /\ match_states s2 s2'.
+  Proof.
+    intros. inv MAT. eapply try_swap_head_not_change in CODE. destruct CODE as [n']. 
+    inv STEP. 
+    (* Lgetstack *)
+    eexists (State _ _ _ _ _ _); split. eapply exec_Lgetstack. eapply eq_refl.
+    inv MEM. eapply match_regular_state; eauto.
+    assert(rs1 (S sl ofs ty) = rs1' (S sl ofs ty)). apply RS.
+    rewrite H. eapply lsagree_set, lsagree_undef_regs. eauto. mem_eq.
+    (* Lsetstack *)
+    eexists (State _ _ _ _ _ _); split. eapply exec_Lsetstack. eapply eq_refl. 
+    eapply match_regular_state; eauto. erewrite lsagree_get; eauto.
+    eapply lsagree_set, lsagree_undef_regs; auto.
+    (* Mop *)
+    inv MEM. eexists (State _ _ _ _ _ _); split. 
+    eapply exec_Lop; eauto. erewrite lsagree_reglist in H9; eauto. 
+    erewrite <- eval_operation_preserved in H9; eauto. 
+    eapply symbols_preserved. eapply match_regular_state; eauto.
+    eapply lsagree_set, lsagree_undef_regs; eauto. mem_eq.
+    (* Mload *)
+    eexists (State _ _ _ _ _ _); split.
+    eapply exec_Lload; inv MEM; eauto. erewrite lsagree_reglist; eauto.
+    erewrite eval_addressing_preserved; eauto. eapply symbols_preserved.
+    eapply lsagree_symmetric; auto. eapply match_regular_state; eauto.
+    eapply lsagree_set, lsagree_undef_regs; eauto.
+    (* Mstore *)
+    inv MEM. eexists (State _ _ _ _ _ _); split.
+    eapply exec_Lstore. erewrite lsagree_reglist; eauto.
+    erewrite eval_addressing_preserved; eauto. eapply symbols_preserved. 
+    eapply lsagree_symmetric; eauto. erewrite <- lsagree_get; eauto.
+    eapply eq_refl. eapply match_regular_state; eauto.
+    (* eapply lsagree_undef_regs; eauto.  *)
+    mem_eq.
+    (* Lcall *)
+    inv MEM. eapply find_function_match in H9 as [cunit [tf []]].
+    erewrite lsagree_find_function in H; eauto.
+    eexists (Callstate _ _ _ _); split. eapply exec_Lcall. eexact H.
+    eapply match_fundef_funsig; eauto. eapply match_call_state; eauto.
+    eapply Forall2_cons; eauto. eapply match_stackframes_intro; eauto.
+    eapply match_fundef_match_fundef0; eauto. mem_eq.
+    (* Ltailcall *)
+    inv MEM. eapply find_function_match in H10 as [cunit [tf []]].
+    erewrite lsagree_find_function in H; eauto.
+    eexists (Callstate _ _ _ _); split. eapply exec_Ltailcall. eapply eq_refl.
+    eexact H. eapply match_fundef_funsig; eauto. simpl; eauto. eapply match_call_state; eauto.
+    eapply match_fundef_match_fundef0; eauto. eapply lsagree_return_regs.
+    inv STK; eauto. eapply lsagree_refl. simpl. destruct x; destruct y; auto. inv H1; auto.
+    auto. mem_eq. eapply lsagree_return_regs. inv STK; eauto. eapply lsagree_refl. simpl.
+    destruct x; destruct y; auto.  inv H1; auto. auto.
+    (* Mbuiltin *)
+    inv MEM. eexists (State _ _ _ _ _ _); split. eapply exec_Lbuiltin.
+    eapply lsagree_eval_builtin_args with (rs:=rs1) in H9. 2: { eauto. }
+    eapply eval_builtin_args_preserved. eapply symbols_preserved. eauto.
+    eapply extcall_genv_irrelevent; eauto. eapply senv_preserved. eauto.
+    eapply match_regular_state; eauto.
+    eapply lsagree_setres. eapply lsagree_undef_regs; eauto. mem_eq.
+    (* Llabel*)
+    eexists (State _ _ _ _ _ _); split. eapply exec_Llabel; eauto.
+    eapply match_regular_state; eauto.
+    (* Lgoto *)
+    pose proof (find_label_try_swap lbl (fn_code fb)) b' n_f H9. destruct H as [nn].
+    eexists (State _ _ _ _ _ _); split. eapply exec_Lgoto. eauto.
+    eapply match_regular_state; eauto.
+    (* Lcond_true *)
+    inv MEM. pose proof (find_label_try_swap lbl (fn_code fb)) b' n_f H11. destruct H as [nn].
+    eexists (State _ _ _ _ _ _); split. eapply exec_Lcond_true. erewrite <- lsagree_reglist; eauto.
+    eapply eq_refl. eauto. eapply match_regular_state; eauto. mem_eq.
+    (* Lcond_false *)
+    inv MEM. eexists (State _ _ _ _ _ _); split. eapply exec_Lcond_false; eauto.
+    erewrite <- lsagree_reglist; eauto. eapply match_regular_state; eauto. mem_eq.
+    (* Lcond_jumptable *)
+    inv MEM. pose proof (find_label_try_swap lbl (fn_code fb)) b' n_f H11. destruct H as [nn].
+    eexists (State _ _ _ _ _ _); split. eapply exec_Ljumptable; eauto.
+    rewrite <- H9; symmetry; eapply lsagree_get; eauto.
+    eapply match_regular_state; eauto. eapply lsagree_undef_regs; eauto. mem_eq.
+    (* Lreturn *)
+    inv MEM. eexists (Returnstate _ _ _); split. eapply exec_Lreturn; eauto.
+    eapply match_return_state; eauto. eapply lsagree_return_regs; eauto.
+    inv STK; eauto. eapply lsagree_refl. simpl. destruct x; destruct y; auto. inv H; auto. mem_eq.
+  Qed.
+
+
+  (** Case 2: Swapped 2 consecutive steps **)
+
+  Lemma set_different_reg: forall res r rs v,
+    res <> r -> Locmap.set (R res) v rs (R r) = rs (R r).
+  Proof. intros. unfold Locmap.set. destruct (Loc.eq (R res) (R r)). inv e; exfalso; auto.
+    destruct (Loc.diff_dec (R res) (R r)); auto.
+    exfalso. apply n0; intro. subst. apply n; auto. Qed.
+
+  Lemma set_different_reglist: forall args dst v rs,
+    mreg_in_list dst args = false ->
+      reglist (Locmap.set (R dst) v rs) args = reglist rs args.
+  Proof. induction args; simpl; intros; auto. eapply orb_false_iff in H as [].
+    erewrite IHargs; eauto. unfold Locmap.set. destruct (Loc.eq (R dst) (R a)).
+    inv e. destruct (mreg_eq a a). inv H. exfalso; apply n; auto.
+    destruct (Loc.diff_dec (R dst) (R a)); auto. exfalso; apply n0. simpl; intro; subst.
+    destruct (mreg_eq a a). inv H. exfalso; apply n; auto. Qed.
+
+  Lemma destroy_not_influenced: forall destroy a rs, 
+    mreg_in_list a destroy = false -> rs (R a) = undef_regs destroy rs (R a).
+  Proof.
+    intro. induction destroy; auto. simpl. intros. apply orb_false_iff in H as [].
+    unfold Locmap.set.
+    destruct (Loc.eq (R a) (R a0)); destruct (Loc.diff_dec (R a) (R a0)); auto.
+    simpl in d. inv e. exfalso; apply d; auto.
+    inv e. destruct (mreg_eq a0 a0). simpl in H. discriminate H. exfalso; apply n0; auto.
+    exfalso. apply n0. simpl. intro; subst. apply n; auto.
+  Qed. 
+
+  Lemma eval_args_irrelevent: forall args rs res0 v0 destroy,
+    mreg_in_list res0 args = false ->
+    mreg_list_intersec args destroy = false ->
+      LTL.reglist rs args =
+      (LTL.reglist (Locmap.set (R res0) v0 (LTL.undef_regs destroy rs)) args).
+  Proof.
+    intro. induction args; auto. intros. simpl in H, H0.
+    rewrite orb_false_iff in H, H0. destruct H, H0. simpl.
+    rewrite <- IHargs; auto.
+    assert( a <> res0 ). simpl in H. destruct mreg_eq. discriminate H. auto.
+    assert(rs (R a) = Locmap.set (R res0) v0 (LTL.undef_regs destroy rs) (R a)).
+    unfold Locmap.set. destruct (Loc.eq (R res0) (R a)). inv e; exfalso; auto.
+    destruct (Loc.diff_dec (R res0) (R a)). 2:{ exfalso. apply n0. simpl. auto. }
+    eapply destroy_not_influenced; auto.
+    rewrite H4; auto.
+  Qed.
+
+  Lemma eval_addressing_irrelevent: forall addr args sp rs res0  v0 destroy,
+    mreg_in_list res0 args = false ->
+    mreg_list_intersec args destroy = false ->
+      eval_addressing ge sp addr (reglist rs args) =
+      eval_addressing ge sp addr
+        (reglist (Locmap.set (R res0) v0 (undef_regs destroy rs)) args).
+  Proof. intros. erewrite <- eval_args_irrelevent; eauto. Qed.
+
+  Lemma not_destroyed_reg: forall destroy rs r,
+    mreg_in_list r destroy = false ->
+    (undef_regs destroy rs) (R r) = rs (R r).
+  Proof.
+    intro; induction destroy; auto. simpl. intros. apply orb_false_iff in H as [].
+    unfold Locmap.set. destruct (Loc.eq (R a) (R r)). exfalso. inv e. destruct (mreg_eq r r); auto. inv H.
+    destruct (Loc.diff_dec (R a) (R r)). 2: { simpl in n0. exfalso. apply n0. intro; subst. apply n; auto. }
+    simpl in d. eapply IHdestroy; eauto.
+  Qed.
+
+  Lemma destroyed_reg: forall destroy rs r,
+    mreg_in_list r destroy = true ->
+    (undef_regs destroy rs) (R r) = Vundef.
+  Proof.
+    intro; induction destroy; auto; simpl; intros. discriminate H.
+    apply orb_true_iff in H as []; unfold Locmap.set.
+    destruct (Loc.eq (R a) (R r)); auto. exfalso. destruct (mreg_eq r a). subst. apply n; auto. inv H.
+    eapply IHdestroy in H. erewrite H.
+    destruct (Loc.eq (R a) (R r)); destruct (Loc.diff_dec (R a) (R r)); auto.
+  Qed.
+
+  Lemma not_destroyed_slot: forall destroy rs sl z ty,
+    (undef_regs destroy rs) (S sl z ty) = rs (S sl z ty).
+  Proof. intro; induction destroy; simpl; auto. Qed.
+
+  Lemma not_destroyed_reglist: forall args destroy rs,
+    mreg_list_intersec args destroy = false ->
+     reglist (undef_regs destroy rs) args = reglist rs args.
+  Proof. induction args; simpl; auto; intros. apply orb_false_iff in H as [].
+    erewrite IHargs; eauto. erewrite not_destroyed_reg; eauto. Qed.
+
+  Lemma lsagree_swap_destroy:
+    forall r res res0 destroy destroy0 rs rs' v v0,
+    lsagree rs rs' -> R res <> r -> R res0 <> r ->
+    mreg_in_list res destroy0 = false ->
+    mreg_in_list res0 destroy = false ->
+    undef_regs destroy0
+    (fun p : loc => if Loc.eq (R res) p then v
+                    else if Loc.diff_dec (R res) p
+                    then undef_regs destroy rs p else Vundef) r
+    = undef_regs destroy
+    (fun p : loc => if Loc.eq (R res0) p then v0
+                    else if Loc.diff_dec (R res0) p 
+                    then undef_regs destroy0 rs' p else Vundef) r.
+  Proof.
+    intros r res res0. destruct r. 
+    { intros. remember (mreg_in_list r destroy0) as b1. remember (mreg_in_list r destroy) as b2.
+      destruct b1; destruct b2; symmetry in Heqb1; symmetry in Heqb2.
+      - erewrite! destroyed_reg; eauto.
+      - erewrite destroyed_reg; eauto. erewrite not_destroyed_reg; eauto.
+        destruct (Loc.eq (R res0) (R r)). inv e. exfalso. apply H1; auto.
+        destruct (Loc.diff_dec (R res0) (R r)); auto. erewrite destroyed_reg; auto.
+      - erewrite not_destroyed_reg; eauto. erewrite! destroyed_reg; eauto.
+        destruct (Loc.eq (R res) (R r)). inv e. exfalso. apply H0; auto.
+        destruct (Loc.diff_dec (R res) (R r)); auto.
+      - erewrite! not_destroyed_reg; eauto.
+        destruct (Loc.eq (R res) (R r)). inv e. exfalso. apply H0; auto.
+        destruct (Loc.eq (R res0) (R r)). inv e. exfalso. apply H1; auto.
+        destruct (Loc.diff_dec (R res) (R r)); destruct (Loc.diff_dec (R res0) (R r)); auto.
+        eapply H. exfalso. apply n1. simpl. intro; subst. apply H1; auto.
+        exfalso. apply n1. simpl. intro; subst. apply H0; auto.
+    }
+    { intros. rewrite! not_destroyed_slot. simpl. eapply H. }
+  Qed.
+
+  Lemma lsagree_indep_set: forall rs rs' res res0 v v0 destroy destroy0,
+    (if mreg_eq res res0 then true else false) = false ->
+    mreg_in_list res destroy0 = false ->
+    mreg_in_list res0 destroy = false ->
+    lsagree rs rs' ->
+    lsagree (Locmap.set (R res0) v0 
+              (undef_regs destroy0 (Locmap.set (R res) v (undef_regs destroy rs))))
+            (Locmap.set (R res) v
+              (undef_regs destroy (Locmap.set (R res0) v0 (undef_regs destroy0 rs')))).
+  Proof.
+    intros. intro. unfold Locmap.get; simpl. unfold Locmap.set.
+    destruct (Loc.eq (R res0) r); destruct (Loc.eq (R res) r).
+    { subst. inv e0. destruct (mreg_eq res0 res0). discriminate H. exfalso; apply n; auto. }
+    { subst. destruct (Loc.diff_dec (R res) (R res0)). simpl in d.
+      erewrite <- destroy_not_influenced; auto. destruct (Loc.eq (R res0) (R res0)); auto.
+      destruct (Loc.diff_dec (R res0) (R res0)); auto.
+      exfalso; apply d0; auto. exfalso; auto. simpl in n0. exfalso; apply n0; intro; subst; auto. }
+    { subst. destruct (Loc.diff_dec (R res0) (R res)). simpl in d.
+      erewrite <- destroy_not_influenced; auto. destruct (Loc.eq (R res) (R res)); auto.
+      destruct (Loc.diff_dec (R res) (R res)); auto.
+      exfalso; apply d0; auto. exfalso; auto. simpl in n0. exfalso; apply n0; intro; subst; auto. }
+    { destruct (Loc.diff_dec (R res0) r).
+      2:{ destruct r. simpl in n1. exfalso; apply n1; intro; subst; auto. simpl in n1; exfalso; auto. }
+      destruct (Loc.diff_dec (R res) r).
+      2:{ destruct r. simpl in n1. exfalso; apply n1; intro; subst; auto. simpl in n1; exfalso; auto. }
+      eapply lsagree_swap_destroy; eauto. }
+  Qed.
+
+  Lemma lsagree_indep_set_destroy: forall rs rs' res v destroy destroy0,
+  mreg_in_list res destroy0 = false ->
+  lsagree rs rs' ->
+  lsagree
+    (undef_regs destroy0 (Locmap.set (R res) v (undef_regs destroy rs)))
+    (Locmap.set (R res) v (undef_regs destroy (undef_regs destroy0 rs'))).
+  Proof.
+    intros. intro. unfold Locmap.get. unfold Locmap.set. destruct (Loc.eq (R res) r).
+    { subst. erewrite not_destroyed_reg; eauto. destruct (Loc.eq (R res) (R res)); auto.
+      exfalso. apply n; auto. }
+    { destruct r.
+      { remember (mreg_in_list r destroy0) as b1. remember (mreg_in_list r destroy) as b2.
+        destruct b1; destruct b2; symmetry in Heqb1; symmetry in Heqb2.
+        - erewrite! destroyed_reg; eauto. destruct (Loc.diff_dec (R res) (R r) ); eauto.
+        - erewrite destroyed_reg; eauto. erewrite not_destroyed_reg; eauto.
+          erewrite destroyed_reg; eauto. destruct (Loc.diff_dec (R res) (R r) ); eauto.
+        - erewrite not_destroyed_reg; eauto.  erewrite destroyed_reg; eauto.
+          erewrite destroyed_reg; eauto. destruct (Loc.eq (R res) (R r)); eauto.
+          inv e; exfalso; apply n; auto.
+        - erewrite! not_destroyed_reg; eauto. destruct (Loc.eq (R res) (R r)); eauto.
+          inv e; exfalso; apply n; auto. destruct (Loc.diff_dec (R res) (R r)); eauto. }
+      erewrite! not_destroyed_slot; eauto. simpl. apply H0. }
+  Qed.
+
+  Lemma independent_two_step_match:
+      forall stk stk' f f' sp sp' c rs rs' m m' s3 i1 i2 t
+      (INDEP: i1 D~> i2 = false)
+      (s1:= State stk f sp (i1::i2::c) rs m)
+      (STEP13: starN step ge 2 s1 t s3)
+      (s1':= State stk' f' sp' (i2::i1::c) rs' m')
+      (MAT: match_states s1 s1'),
+        exists s3', tPlus s1' t s3' /\ match_states s3 s3'.
+  Proof.
+    intros. inv STEP13. rename s' into s2. inv H1. inv H3. rename t0 into t2.
+    assert(B:forall b b1: bool, (if b then b1 else b1) = b1). intros; destruct b; auto.
+    assert(Hstep12 := H0). assert(Hstep23 := H2). set(s2_ := s2). set(s3_ := s3).
+    (* 13 branches in total need to reason dependences; others can be discriminated instinctly *)
+    inv H0; inv H2; unfold happens_before in INDEP; simpl in INDEP; 
+      try discriminate INDEP; repeat apply orb_false_iff in INDEP as [INDEP ?];
+      rename INDEP into RW; rename H into DES; rename H0 into MM;
+      try rename H1 into WW; try rename H2 into WR;
+      repeat apply orb_false_iff in DES as [DES]; rename H1 into DES0;
+      rename H0 into DES1; rename H into DES2;
+      fold s2_ in Hstep12, Hstep23; fold s3_ in Hstep23.
+    (* Lgetstack D~> i2: trivial & discriminated *)
+    (* Msetstack D~> i2: trivial & discriminated *) (* Msetstack D~> Mop *)
+    (* Lop D~> i2 *) (* Lop D~> Lgetstack  *) (* Lop D~> Lset  *) (* Lop D~> Lgetparam: discriminated *)
+        (* Lop D~> Lop *)
+    + set(f'_ := f'). inv MAT. inv MEM. rename sp' into sp. rename m' into m.
+      simpl in RW, WR, WW. unfold hb_ww in WW; simpl in WW. assert(WW_:= WW).
+      destruct (mreg_eq res res0) in WW; try discriminate WW.
+      unfold hb_rw, hb_wr in RW; simpl in RW.
+      erewrite <- eval_args_irrelevent in H9; eauto.
+      erewrite eval_args_irrelevent in H10; eauto.
+      eassert(Hstep12': step tge s1' E0 _). eapply exec_Lop; eauto.
+      erewrite <- lsagree_reglist; eauto.
+      unfold ge in H9; erewrite eval_op_genv_irrelevent in H9; eauto; eapply symbols_preserved.
+      eassert(Hstep23': step tge _ E0 _). eapply exec_Lop; eauto.
+      unfold ge in H10; erewrite eval_op_genv_irrelevent in H10.
+      erewrite <- lsagree_reglist; eauto.
+      eapply lsagree_set, lsagree_undef_regs; eauto. eapply symbols_preserved. 
+      eexists _; split. eapply plus_two; eauto. eapply match_regular_state; eauto.
+      eapply try_swap_at_tail. unfold hb_destroy_dst in DES1, DES2; simpl in DES1, DES2.
+      eapply lsagree_indep_set; eauto. mem_eq.
+    (* Lop D~> Lload *)
+    + set(f'_ := f'). inv MAT. inv MEM. rename sp' into sp. rename m' into m.
+      simpl in RW, WR, WW. unfold hb_ww in WW; simpl in WW. assert(WW_:= WW).
+      unfold hb_rw, hb_wr in RW; simpl in RW.
+      destruct (mreg_eq res dst) in WW; try discriminate WW.
+      erewrite <- eval_addressing_irrelevent in H9; eauto.
+      erewrite eval_args_irrelevent in H10; eauto.
+      eassert(Hstep12': step tge s1' E0 _). eapply exec_Lload; eauto.
+      erewrite <- lsagree_reglist; eauto.
+      unfold ge in H9; erewrite eval_addr_genv_irrelevent in H9; eauto; eapply symbols_preserved.
+      eassert(Hstep23': step tge _ E0 _). eapply exec_Lop; eauto.
+      unfold ge in H10; erewrite eval_op_genv_irrelevent in H10.
+      erewrite <- lsagree_reglist; eauto.
+      eapply lsagree_set, lsagree_undef_regs; eauto. eapply symbols_preserved.
+      eexists _; split. eapply plus_two; eauto. eapply match_regular_state; eauto.
+      eapply try_swap_at_tail. unfold hb_destroy_dst in DES1, DES2; simpl in DES1, DES2.
+      eapply lsagree_indep_set; eauto. mem_eq.
+    (* Lop D~> Lstore *)
+    + fold mreg_in_list in WR. rename WR into RW'. set(f'_ := f').
+      inv MAT. inv MEM. rename sp' into sp. rename m' into m.
+      unfold hb_destroy_src in DES, DES0. simpl in DES, DES0. eapply orb_false_iff in DES0 as [D0 D0'].
+      erewrite <- eval_addressing_irrelevent in H9; eauto.
+      eassert(Hstep12': step tge s1' E0 _). eapply exec_Lstore; eauto.
+      erewrite <- lsagree_reglist; eauto.
+      unfold ge in H9; erewrite eval_addr_genv_irrelevent in H9; eauto; eapply symbols_preserved.
+      erewrite <- H11. erewrite set_different_reg.
+      erewrite not_destroyed_reg; eauto. erewrite <- lsagree_get; eauto.
+      destruct (mreg_eq res src); auto. inv RW.
+      set(s2':= State stk' (try_swap_nth_func n_f f) sp
+                  (Lop op args res :: c)
+                    (undef_regs (destroyed_by_store chunk addr) rs') m'0).
+      eassert(Hstep23': step tge s2' E0 _). eapply exec_Lop; eauto.
+      unfold ge in H10; erewrite eval_op_genv_irrelevent, eval_op_mem_irrelevant in H10.
+      erewrite not_destroyed_reglist. erewrite <- lsagree_reglist; eauto. eauto.
+      unfold hb_mem in MM; simpl in MM. destruct (mem_read_op op); auto. eapply symbols_preserved.
+      eexists _; split. eapply plus_two; eauto. eapply match_regular_state; eauto.
+      eapply try_swap_at_tail. eapply lsagree_indep_set_destroy; eauto. mem_eq.
+  (* Lload D~> i2 *)
+    (* Lload D~> Lgetstack *)  (* Lload D~> Lgetparam *)
+    (* Lload D~> Lop *)
+    + set(f'_ := f'). inv MAT. inv MEM. rename sp' into sp. rename m' into m.
+      simpl in RW, WR, WW. unfold hb_ww in WW; simpl in WW. assert(WW_:= WW).
+      unfold hb_rw, hb_wr in RW; simpl in RW. destruct (mreg_eq dst res) in WW; try discriminate WW.
+      erewrite <- eval_args_irrelevent in H9; eauto.
+      erewrite eval_addressing_irrelevent in H10; eauto.
+      eassert(Hstep12': step tge s1' E0 _). eapply exec_Lop; eauto.
+      erewrite <- lsagree_reglist; eauto.
+      unfold ge in H9; erewrite eval_op_genv_irrelevent in H9; eauto; eapply symbols_preserved.
+      eassert(Hstep23': step tge _ E0 _). eapply exec_Lload; eauto.
+      unfold ge in H10; erewrite eval_addr_genv_irrelevent in H10.
+      erewrite <- lsagree_reglist; eauto.
+      eapply lsagree_set, lsagree_undef_regs; eauto. eapply symbols_preserved.
+      eexists _; split. eapply plus_two; eauto. eapply match_regular_state; eauto.
+      eapply try_swap_at_tail. unfold hb_destroy_dst in DES1, DES2; simpl in DES1, DES2.
+      eapply lsagree_indep_set; eauto. mem_eq.
+    (* Lload D~> Lload *)
+    + set(f'_ := f'). inv MAT. inv MEM. rename sp' into sp. rename m' into m.
+      simpl in RW, WR, WW. unfold hb_ww in WW; simpl in WW. assert(WW_:= WW).
+      destruct (mreg_eq dst dst0) in WW; try discriminate WW.
+      unfold hb_rw, hb_wr in RW; simpl in RW.
+      erewrite <- eval_addressing_irrelevent in H9; eauto.
+      erewrite eval_addressing_irrelevent in H10; eauto.
+      set(s2' := State stk' f'_ sp (Lload chunk addr args dst :: c)
+        (Locmap.set (R dst0) v0 (undef_regs (destroyed_by_load chunk0 addr0) rs')) m).
+      eassert(Hstep12': step tge s1' E0 s2'). eapply exec_Lload; eauto.
+      erewrite <- lsagree_reglist; eauto.
+      unfold ge in H9; erewrite eval_addr_genv_irrelevent in H9; eauto.
+      eapply symbols_preserved.
+      eassert(Hstep23': step tge s2' E0 _). eapply exec_Lload; eauto.
+      unfold ge in H10; erewrite eval_addr_genv_irrelevent in H10.
+      erewrite <- lsagree_reglist; eauto.
+      eapply lsagree_set, lsagree_undef_regs; eauto. eapply symbols_preserved.
+      set(s3' := State stk' f'_ sp c
+            (Locmap.set (R dst) v
+              (undef_regs (destroyed_by_load chunk addr)
+                  (Locmap.set (R dst0) v0
+                    (undef_regs (destroyed_by_load chunk0 addr0)
+                        rs')))) m ).
+      exists s3'; split. eapply plus_two; eauto. eapply match_regular_state; eauto.
+      reflexivity. eapply try_swap_at_tail. unfold hb_destroy_dst in DES1, DES2; simpl in DES1, DES2.
+      eapply lsagree_indep_set; eauto. reflexivity.
+  (* Lload D~> Lstore: discriminated because alias analysis is not supported *)
+    + unfold hb_mem in MM; simpl in MM. discriminate MM.
+  (* Lstore D~> i2: *)
+    (* Lstore D~> Lop *)
+    + fold mreg_in_list in H3. fold mreg_list_intersec in H2. set(f'_ := f').
+      inv MAT. inv MEM. rename sp' into sp. rename m' into m.
+      unfold hb_destroy_src in DES, DES0. simpl in DES, DES0.
+      erewrite eval_addressing_irrelevent in H10; eauto.
+      eassert(Hstep12': step tge s1' E0 _). eapply exec_Lop; eauto.
+      unfold ge in H9; erewrite eval_op_genv_irrelevent, eval_op_mem_irrelevant in H9.
+      erewrite <- H9.
+      erewrite not_destroyed_reglist; eauto. erewrite <- lsagree_reglist; eauto. eapply eq_refl.
+      unfold hb_mem in MM; simpl in MM. destruct (mem_read_op op); auto. eapply symbols_preserved.
+      set(s2':= State stk' (try_swap_nth_func n_f f) sp
+                  (Lstore chunk addr args src :: c)
+                  (Locmap.set (R res) v (undef_regs (destroyed_by_op op) rs'))
+                  m).
+      eassert(Hstep23': step tge s2' E0 _). eapply exec_Lstore; eauto.
+      unfold ge in H10; erewrite eval_addr_genv_irrelevent in H10. 
+      erewrite <- H10. instantiate (1:= v). instantiate (1:= tprog). simpl.
+      erewrite <- lsagree_reglist; eauto. eapply lsagree_set, lsagree_undef_regs; eauto.
+      eapply symbols_preserved. erewrite set_different_reg; eauto.
+      erewrite not_destroyed_reg; eauto. erewrite <- lsagree_get; eauto.
+      destruct (mreg_eq res src); auto. inv RW. 
+      eexists _; split. eapply plus_two; eauto. eapply match_regular_state; eauto.
+      eapply try_swap_at_tail. eapply lsagree_symmetric. eapply lsagree_indep_set_destroy; eauto.
+      eapply lsagree_symmetric; eauto. mem_eq.
+    (* Lstore D~> Lload *)
+    + unfold hb_mem in MM; simpl in MM. discriminate MM.
+  (* Lcall D~> i2: trivial & discriminated *) (* Ltailcall D~> i2: trivial & discriminated *)
+  (* Lbuiltin D~> i2: trivial & discriminated *) (* Lgoto D~> i2: trivial & discriminated *)
+  (* Lcond D~> i2: trivial & discriminated*)
+  Qed.
+
+  Definition next_exec (s: state): option instruction :=
+    match s with
+    (* | State _ _ _ (Lreturn :: _) _ _ => None *)
+    | State _ _ _ (i :: _) _ _ => Some i
+    | _ => None
+    end.
+
+  Definition index := option instruction.
+  Inductive orderb: index -> index -> Prop :=
+    | orderb_neq: forall i, orderb (Some i) None.
+
+  Lemma wf_orderb: well_founded orderb.
+  Proof. hnf. intros. eapply Acc_intro. intros.
+    induction H. eapply Acc_intro. intros. inv H. Qed.
+
+    (*
+       sa ~~~~~~~> sb
+        |         /
+        |       /
+  match |     / aux. match
+        |   /
+        | /
+        sa'
+  *)
+  Inductive match_states_aux: index -> state -> state -> Prop :=
+  | match_now : forall s s', match_states s s' -> match_states_aux None s s'
+  | match_before: 
+      forall sa i sa' t sb,
+        next_exec sa = Some i -> solid_inst i = false ->
+        step ge sa t sb -> match_states sa sa' -> 
+          match_states_aux (Some i) sb sa'
+  .
+
+  Lemma simulation:
+    forall s1 t s2, step ge s1 t s2 -> 
+      forall b s1', match_states_aux b s1 s1' ->
+        exists b', exists s2', 
+          (tPlus s1' t s2' \/ (tStar s1' t s2' /\ orderb b' b) ) 
+        /\ match_states_aux b' s2 s2'. 
+  Proof.
+    intros. inv H0.
+    - (* match now *)
+      set (s1'_:=s1'). assert (Hm:= H1). inv H1.
+      + (* regular state *) destruct c as [ | i1]. inv H.
+        destruct c as [|i2 c].
+        (* only one inst left - one step matching *)
+        { edestruct regular_state_one_step_match.
+          eapply H. eapply match_regular_state; eauto. eapply try_swap_at_tail.
+          eexists None, x. destruct H0. split; left; eauto. eapply plus_one.  
+          erewrite <- try_swap_singleton in H0; eauto. }
+        (* may be a swapping *)
+        destruct n_c.
+        (* try swapping now *)
+        { simpl in *. remember (i1 D~> i2) as INDEP; symmetry in HeqINDEP. destruct INDEP.
+          (* swapping failed, one step matching*)
+          { edestruct regular_state_one_step_match. eapply H. 
+            eapply match_regular_state; eauto.
+            eapply try_swap_at_tail. destruct H0. 
+            exists None, x; eauto. split; left; eauto. eapply plus_one; eauto. }
+          (* swapping succeeded, delayed mathching *)
+          { eexists (Some i1), s1'_. split. right; eauto; simpl. split. 
+            assert (t = E0). { inv H; auto; simpl in HeqINDEP. discriminate HeqINDEP. } 
+            subst. eapply star_refl. eapply orderb_neq.
+            eapply match_before; eauto. auto.
+            eapply indep_inv_not_solid1; eauto.
+          }
+        }
+        (* try swapping later *)
+        { simpl in *. edestruct regular_state_one_step_match. eapply H. 
+        eapply match_regular_state; eauto. instantiate(2:=Datatypes.S n_c).
+        simpl. eapply eq_refl. destruct H0. 
+        exists None, x; eauto. split; left; eauto. eapply plus_one; eauto. }
+      + (* call state, one step matching *) 
+        inv H.
+        (* call internal *)
+        { inv MEM. inv FUNC. eexists None, (State _ _ _ _ _ _). split.
+          left. eapply plus_one.
+          eapply exec_function_internal; eauto. eapply match_now.
+          eapply match_regular_state; eauto. simpl. eapply eq_refl.
+          eapply lsagree_undef_regs, lsagree_call_regs; auto. mem_eq. }
+        (* call external *)
+        { inv MEM. inv FUNC. eexists None, (Returnstate _ _ _). split.
+          left. eapply plus_one. eapply exec_function_external; eauto.
+          eapply extcall_genv_irrelevent in H7.
+          assert( forall l, map (fun p => Locmap.getpair p rs) l = map (fun p=> Locmap.getpair p rs') l).
+          { induction l; auto. simpl. erewrite lsagree_getpair; eauto. erewrite IHl; eauto. }
+          erewrite H in H7. eauto. eapply senv_preserved. eapply match_now.
+          eapply match_return_state; eauto. eapply lsagree_setpair. 
+          eapply lsagree_undef_caller_save_regs; auto. mem_eq. }
+      + (* return state, one step matching *)
+        inv H. inv MEM. inv STL. inv H1.
+        eexists None, (State _ _ _ _ _ _); split; left. eapply plus_one. 
+        eapply exec_return. eapply match_regular_state; eauto. mem_eq.
+    - (* match before *)
+                (*
+              sa ~~~~~~~> s1 ~~~~~~~> s2
+                |         /
+                |       /
+          match |     / aux. match
+                |   /
+                | /
+                s1'
+                *)
+      set(sa_ := sa). assert(Hm:= H4). inv H4.
+      + (* regular state *) rename i into i1.
+        destruct c; simpl in H1. discriminate H1. inv H1. destruct c as [|i2 c].
+        (* only one inst left but not a return - impossible *)
+        {
+          eapply exec_one_inst in H3 as [sl1 [f1 [sp1 [rs1 [m1]]]]].
+          subst. inv H. auto. }
+        (* more than two inst left,  *)
+        destruct n_c.
+        (* i1 i2 may be two swapped inst *)
+        { simpl in *. remember (i1 D~> i2) as HB12. symmetry in HeqHB12. destruct HB12.
+          (* i1 i2 not swapped *)
+          { edestruct regular_state_one_step_match. eapply H3. eapply Hm. destruct H0.
+          assert(Hstep'12:=H0).
+          eapply exec_one_inst in H3 as [sl1 [f1 [sp1 [rs1 [m1]]]]]; eauto. subst.
+          eapply exec_one_inst in H0 as [sl1' [f1' [sp1' [rs1' [m1']]]]]; eauto. subst.
+          edestruct regular_state_one_step_match. eapply H. eapply H1. destruct H0.
+          exists None, x. split; left; auto. eapply plus_two; eauto.
+          assert(t0 = E0). { inv Hstep'12; auto. discriminate H2. } subst.
+          eapply E0_left. }
+          (* i1 i2 was swapped, use previous lemma *)
+          { edestruct independent_two_step_match; eauto.
+            repeat eapply starN_step; eauto. eapply starN_refl.
+            exists None, x. destruct H0. split; left; eauto.
+            assert(t0 = E0). { inv H3; auto. discriminate H2. } subst.
+            erewrite E0_right, E0_left in H0; auto.
+            }
+        }
+        (*  i2 i3 not swapped here *)
+        { simpl in *. edestruct regular_state_one_step_match. eapply H3. eapply Hm.
+          destruct H0. destruct c as [| i3 c].
+          (* i2 i3 not swapped here, either *)
+          { erewrite try_swap_code_singleton in H0.
+            eapply exec_one_inst in H3 as [sl1 [f1 [sp1 [rs1 [m1]]]]]; eauto. subst.
+            assert(Hm1:= H1). inv H1. erewrite try_swap_code_singleton in Hm1.
+            edestruct regular_state_one_step_match. eapply H. eapply Hm1.
+            destruct H1. exists None, x. split; left; eauto.
+            erewrite try_swap_code_singleton. erewrite try_swap_code_singleton in H0. 
+            eapply plus_two; eauto.
+            assert(t0 = E0). { inv H0; auto. discriminate H2. } subst.
+            apply E0_left. }
+          (* i2 i3 may be swapped *)
+          { destruct n_c.
+            { simpl in *. remember (i2 D~> i3) as HB23.
+              destruct HB23; symmetry in HeqHB23.
+              (* i2 i3 not swapped *)
+              { assert(Hstep0 := H0). 
+                eapply exec_one_inst in H0 as [sl1' [f1' [sp1' [rs1' [m1']]]]]; eauto. subst.
+                eapply exec_one_inst in H3 as [sl1 [f1 [sp1 [rs1 [m1]]]]]; eauto. subst.
+                edestruct regular_state_one_step_match. eapply H. eapply H1.
+                destruct H0. exists None, x. split; left; eauto. 
+                eapply plus_two; eauto. assert(t0 = E0). 
+                { inv Hstep0; auto. discriminate H2. } subst. apply E0_left. }
+              (* i2 i3 was swapped *)
+              { exists (Some i2), x. eapply indep_inv_not_solid1 in HeqHB23.
+                eapply exec_one_inst in H3 as [sl1 [f1 [sp1 [rs1 [m1]]]]]; eauto. subst.
+                split. left. eapply plus_one.
+                assert(t0 = E0). { inv H0; auto. discriminate H2. } subst.
+                assert(t = E0). { inv H; auto. discriminate HeqHB23. } subst.
+                auto. eapply match_before; eauto; auto. 
+              }
+            }
+            { simpl in *. assert(Hstep0 := H0). 
+              eapply exec_one_inst in H0 as [sl1' [f1' [sp1' [rs1' [m1']]]]]; eauto. subst.
+              eapply exec_one_inst in H3 as [sl1 [f1 [sp1 [rs1 [m1]]]]]; eauto. subst.
+              edestruct regular_state_one_step_match. eapply H. eapply H1.
+              destruct H0. exists None, x. split; left; eauto. 
+              eapply plus_two; eauto. assert(t0 = E0). 
+              { inv Hstep0; auto. discriminate H2. } subst. apply E0_left.
+            } 
+          }
+       }
+      + (* call state *) simpl in H1; discriminate H1.
+      + (* return state *) simpl in H1; discriminate H1.
+  Qed.
+
+  Lemma transf_initial_states:
+    forall st1, initial_state prog st1 ->
+    exists b st2, initial_state tprog st2 /\ match_states_aux b st1 st2.
+  Proof.
+    intros. inv H.
+    eapply (Genv.find_funct_ptr_match TRANSF) in H2; eauto.
+    destruct H2 as [cu [tf [? []]]]. inv H2.
+    - exists None, (Callstate [] (Internal ((try_swap_nth_func n f0))) (Locmap.init Vundef) m0).
+      split. eapply initial_state_intro; eauto.
+      eapply (Genv.init_mem_match TRANSF); trivial. 
+      rewrite (match_program_main TRANSF); rewrite symbols_preserved; auto.
+      eapply match_now, match_call_state; eauto. eapply Forall2_nil.
+      eapply match_fundef0_internal. eapply lsagree_refl. reflexivity.
+    - exists None, (Callstate [] (External f0)  (Locmap.init Vundef) m0).
+      split. eapply initial_state_intro; eauto.
+      eapply (Genv.init_mem_match TRANSF); trivial. 
+      rewrite (match_program_main TRANSF); rewrite symbols_preserved; auto.
+      eapply match_now, match_call_state; eauto. eapply Forall2_nil.
+      eapply match_fundef0_external. eapply lsagree_refl. reflexivity.
+  Qed.
+
+  Lemma transf_final_states0:
+    forall st1 st2 r,
+    match_states st1 st2 -> final_state st1 r -> final_state st2 r.
+  Proof. 
+    intros. inv H0. inv H. inv STL.
+    eapply final_state_intro. 
+    erewrite <- lsagree_getpair; eauto.
+  Qed.
+
+  Lemma transf_final_states:
+    forall b st1 st2 r,
+    match_states_aux b st1 st2 -> final_state st1 r -> final_state st2 r.
+  Proof.
+    intros. inv H.
+    - (* match now *)
+      eapply transf_final_states0; eauto.
+    - (* match before, not possible *)
+      inv H0. inv H3; simpl in H1; inv H1; discriminate H2.
+  Qed.
+
+  Theorem forward_simulation_safe_swap:
+    forward_simulation (Linear.semantics prog) 
+                       (Linear.semantics tprog).
+  Proof.
+    eapply Forward_simulation with orderb match_states_aux; constructor.
+    - apply wf_orderb.
+    - apply transf_initial_states.
+    - apply transf_final_states.
+    - apply simulation.
+    - apply senv_preserved.
+  Qed.
+
+End SINGLE_SWAP_CORRECTNESS.
+
+
+Lemma transf_program_single_swap_forward_simulation:
+  forall pos n prog tprog, 
+    transf_program_try_swap_in_one pos n prog = OK tprog ->
+    forward_simulation (Linear.semantics prog) (Linear.semantics tprog).
+Proof.
+  intros. eapply forward_simulation_safe_swap.
+  eapply transf_program_match; eauto.
+Qed.
+
+
+Lemma transf_program_multi_swap_forward_simulation:
+  forall seq prog tprog,
+  transf_program_try_swap_seq seq prog = OK tprog ->
+    forward_simulation (Linear.semantics prog) (Linear.semantics tprog).
+Proof.
+  induction seq.
+  - intros. inv H. destruct prog; apply forward_simulation_refl.
+  - intros. destruct prog. destruct a as [pos n]. 
+  unfold transf_program_try_swap_seq in H; simpl in H. inv H.
+  set (prog' := {|
+      prog_defs := try_swap_prog_def_in_one pos n prog_defs;
+      prog_public := prog_public;
+      prog_main := prog_main
+    |}).
+  eapply compose_forward_simulations with (L2:= semantics prog'); auto.
+  eapply transf_program_single_swap_forward_simulation; unfold prog'.
+  unfold transf_program_try_swap_in_one; eauto.
+Qed.
+
+(* [pos1, n1] :: [pos2, n2] :: ... 
+   1st aug: try swap at which program definition (do nothing if not a internal function)
+   2nd aug: try swap at which location of that funtion's code *)
+Fixpoint transf_program_try_swap_seq1 (seq: list (nat * nat) ) (prog: program):=
+  match seq with
+  | [] => OK prog
+  | (pos, n) :: seq' => do prog' <- transf_program_try_swap_in_one pos n prog;
+                       transf_program_try_swap_seq1 seq' prog'
+  end.
+
+Lemma transf_program_multi_swap_forward_simulation1:
+  forall seq prog tprog, 
+  transf_program_try_swap_seq1 seq prog = OK tprog ->
+    forward_simulation (Linear.semantics prog) (Linear.semantics tprog).
+Proof.
+  induction seq.
+  - intros. inv H. apply forward_simulation_refl.
+  - intros. simpl in H. destruct a as [pos n].
+    eapply IHseq in H.
+    set (prog' := {|
+      prog_defs := try_swap_prog_def_in_one pos n (prog_defs prog);
+      prog_public := prog_public prog;
+      prog_main := prog_main prog
+    |}). fold prog' in H.
+    eapply compose_forward_simulations with (L2:= semantics prog'); auto. 
+    eapply transf_program_single_swap_forward_simulation; eauto.
+    unfold transf_program_try_swap_in_one. unfold prog'. eauto.
+Qed.
+
+
+Section ABSTRACT_SCHEDULER.
+
+  Variable schedule': list (positive * instruction) -> res (list (positive * instruction)).
+
+  Let HBR := fun i1 i2 => happens_before i1 i2 = true.
+  Let HBnum (na1 na2: positive * instruction) := happens_before (snd na1) (snd na2).
+  Let HBGenR (l: list instruction) := GenR HBR l.
+
+  Hypothesis schedule_valid:
+    forall l nl', schedule' (numlistgen l) = OK nl' -> 
+      treorder HBR l (numlistgen l) nl'.
+  
+  Definition schedule (l: list instruction): res (list instruction) :=
+    do nl' <- schedule' (numlistgen l);
+    OK (numlistoff nl').
+
+  Definition schedule_function (f: function):=
+    do code' <- schedule (f.(fn_code));
+    OK (mkfunction f.(fn_sig) f.(fn_stacksize) code') .
+
+  Definition schedule_fundef (f: fundef): res fundef :=
+    AST.transf_partial_fundef schedule_function f.
+
+  Definition schedule_program (p: program): res program :=
+    transform_partial_program2 
+    (fun i f => schedule_fundef f) (fun i v => OK v) p.
+
+  Lemma swapping_lemma_numblock:
+    forall l nl', schedule' (numlistgen l) = OK nl' ->
+      exists ln, nl' = try_swap_seq HBnum ln (numlistgen l).
+  Proof.
+    intros. pose proof schedule_valid l.
+    unfold treorder in H0.
+    eapply swapping_property in H0 as [ln]; eauto.
+    intros; rewrite happens_before_symmetric; auto.
+  Qed.
+
+  Lemma swapping_lemma_block: 
+    forall l l', schedule l = OK l' -> exists ln, l' = try_swap_seq happens_before ln l.
+  Proof.
+    intros. monadInv H. edestruct swapping_lemma_numblock as [ln]; eauto.
+    exists ln. erewrite H. eapply try_swap_seq_num_equally.
+  Qed.
+
+  Lemma schedule_program_swapping_lemma_prepare1:
+    forall seq def prog_defs,
+    let seq':= map (fun x => ((Datatypes.S (fst x)), snd x)) seq in
+    try_swap_prog_def_seq seq' (def :: prog_defs)
+     = def :: (try_swap_prog_def_seq seq prog_defs).
+  Proof.
+    induction seq.
+    - intros. simpl; auto.
+    - intros. destruct a as [pos n]. simpl in seq'. unfold seq'. simpl.
+      erewrite IHseq; eauto.
+  Qed.
+
+  Lemma schedule_program_swapping_lemma_prepare2:
+  forall ln prog_defs i f,
+    let seq := List.map (fun n => (O, n)) ln in
+    let prog_defs':= (i, Gfun (Internal f)) :: prog_defs in
+    let prog_defs'' := 
+    (i, Gfun (Internal {| fn_sig := fn_sig f;
+                          fn_stacksize := fn_stacksize f;
+                          fn_code := try_swap_seq happens_before ln (fn_code f) |}))
+    :: prog_defs in
+      try_swap_prog_def_seq seq prog_defs' = prog_defs''.
+  Proof.
+    induction ln.
+    - intros. unfold prog_defs', prog_defs''. simpl; destruct f; auto.
+    - intros. simpl in seq. unfold seq. 
+      unfold prog_defs'. simpl. unfold prog_defs''. simpl.
+      erewrite IHln; eauto.
+  Qed.
+
+  Lemma schedule_program_swapping_lemma_prepare3:
+  forall seq seq' prog_defs prog_defs' prog_defs'', 
+    try_swap_prog_def_seq seq prog_defs = prog_defs' ->
+      try_swap_prog_def_seq seq' prog_defs' = prog_defs'' ->
+        try_swap_prog_def_seq (seq ++ seq') prog_defs = prog_defs''.
+  Proof.
+    intro; induction seq; intros.
+    - simpl in *. subst; auto.
+    - destruct a as [pos n]. simpl in *. eapply IHseq; eauto.
+  Qed.
+
+  Lemma schedule_program_swapping_lemma:
+  forall prog tprog: program, schedule_program prog = OK tprog -> 
+    exists seq: list (nat * nat), transf_program_try_swap_seq seq prog = OK tprog.
+  Proof.
+    intros prog. destruct prog. induction prog_defs.
+    - intros. exists []. simpl. unfold transf_program_try_swap_seq; simpl; auto.
+    - intros. unfold schedule_program in H. monadInv H.
+      destruct a. destruct g. destruct f.
+      { simpl in EQ. 
+        remember (do f' <- schedule_function f; OK (Internal f')) as res.
+        destruct res. 2: inv EQ. 
+        monadInv EQ. inv Heqres. symmetry in H0. monadInv H0.
+        set(prog' :={| prog_defs := x0; prog_public := prog_public;
+          prog_main := prog_main |}).
+        specialize (IHprog_defs prog'). destruct IHprog_defs as [seq0]; auto.
+        unfold schedule_program. unfold transform_partial_program2. simpl.
+        rewrite EQ0; simpl; auto.
+        inv H. set(seq0' := List.map (fun x => (Datatypes.S (fst x), snd x)) seq0 ).
+        pose proof swapping_lemma_block (fn_code f) as [ln]; eauto.
+
+        instantiate (1 := fn_code x). unfold schedule_function in EQ.
+        monadInv EQ. erewrite EQ1; eauto.
+
+        (* unfold schedule_function in EQ.
+        monadInv EQ. *)
+
+        set(seq1 := List.map (fun n => (O, n)) ln).
+        exists (seq0' ++ seq1).
+        unfold transf_program_try_swap_seq; simpl.
+        set(prog_defs0 := (i, Gfun (Internal f)) :: prog_defs).
+        set (prog_defs1 := (i, Gfun (Internal f))  :: try_swap_prog_def_seq seq0 prog_defs).
+        set(prog_defs2 := (i,
+                  Gfun
+                    (Internal
+                      {|
+                        fn_sig := fn_sig f;
+                        fn_stacksize := fn_stacksize f;
+                        fn_code := try_swap_seq happens_before ln (fn_code f)
+                      |})) :: try_swap_prog_def_seq seq0 prog_defs
+        ).
+        assert(try_swap_prog_def_seq seq0' prog_defs0 = prog_defs1).
+        { eapply schedule_program_swapping_lemma_prepare1. }
+        assert(try_swap_prog_def_seq seq1 prog_defs1 = prog_defs2).
+        eapply schedule_program_swapping_lemma_prepare2; eauto.
+        erewrite schedule_program_swapping_lemma_prepare3; eauto.
+        erewrite H1. unfold prog_defs2. unfold schedule_function in EQ.
+        monadInv EQ. simpl in H. subst; eauto.
+      }
+      { simpl in EQ. monadInv EQ.
+        set(prog' :={| prog_defs := x0; prog_public := prog_public;
+        prog_main := prog_main |}).
+        specialize (IHprog_defs prog'). destruct IHprog_defs as [seq0]; auto.
+        unfold schedule_program. unfold transform_partial_program2. simpl.
+        rewrite EQ0; simpl; auto.
+        inv H. set(seq0' := List.map (fun x => (Datatypes.S (fst x), snd x)) seq0 ).
+        exists (seq0').
+        unfold transf_program_try_swap_seq; simpl.
+        erewrite <- schedule_program_swapping_lemma_prepare1; eauto.
+      }
+      { simpl in EQ. monadInv EQ.
+        set(prog' :={| prog_defs := x0; prog_public := prog_public;
+        prog_main := prog_main |}).
+        specialize (IHprog_defs prog'). destruct IHprog_defs as [seq0]; auto.
+        unfold schedule_program. unfold transform_partial_program2. simpl.
+        rewrite EQ0; simpl; auto.
+        inv H. set(seq0' := List.map (fun x => (Datatypes.S (fst x), snd x)) seq0 ).
+        exists (seq0'). 
+        assert(V: v = {|
+          gvar_info := gvar_info v;
+          gvar_init := gvar_init v;
+          gvar_readonly := gvar_readonly v;
+          gvar_volatile := gvar_volatile v
+        |}). destruct v; auto. rewrite <- V.
+        erewrite <- schedule_program_swapping_lemma_prepare1; eauto.
+      }
+  Qed.
+  
+  Theorem schedule_program_forward_simulation:
+    forall prog tprog: program, schedule_program prog = OK tprog ->
+      forward_simulation (Linear.semantics prog) (Linear.semantics tprog).
+  Proof.
+    intros. apply schedule_program_swapping_lemma in H as [seq].
+    eapply transf_program_multi_swap_forward_simulation; eauto.
+  Qed.
+
+End ABSTRACT_SCHEDULER.
+
+Check schedule_program_forward_simulation.
+
+
+(* Case Study: List Scheduling *)
+
+Require Import FSets.
+
+Module PS <: FSetInterface.S := PositiveSet.
+Print Module PS.
+Print PS.elt.
+
+Goal PositiveSet.t = PS.t. unfold PS.t, PositiveSet.t. auto. Qed.
+
+Definition numblock := list (positive * instruction).
+
+Section ABSTRACT_LIST_SCHEDULER.
+
+  (* Some outside priority funcion. The prioirty oracle can be custumized.
+        It should return the location of the first pick *)
+  (* Variable firstpick':
+    list (positive * instruction) -> (* already scheduled instruction*)
+      list (positive * instruction) ->  (* valid to schedule as next instruction *)
+        list (positive * instruction) ->  (* full original codes in the function *)
+          option positive.    *)
+          (* which one in valid-instrucion-list (2nd augument) to pick next *)
+
+  (* Definition firstpick:
+    list (positive * instruction) -> (* already scheduled instruction*)
+      list (positive * instruction) ->  (* valid to schedule as next instruction *)
+        list (positive * instruction) ->  (* full original codes in the function *)
+          positive * instruction.   (* which one in valid-instrucion-list (2nd augument) to pick next *)
+  Admitted. *)
+
+  Variable prioritizer: list instruction -> list positive.
+
+  (* Fixpoint prior_map (pos: positive) (l: list instruction) :=
+    match prioritizer l with
+    | nil =>
+    |  *)
+
+  Check prioritizer.
+
+  (* Temporary *)
+  Definition firstpick (l: list (positive * instruction)) :=
+    match l with
+    | nil => Error (msg "Unexpected Error: Empty available inst to be scheduled")
+    | pi :: l' => OK pi
+    end.
+
+  
+
+  Lemma firstpick_sound: forall nl pi, firstpick nl = OK pi -> In pi nl.
+  Proof. Admitted.
+
+  (* Definition firstpick (l1 l2 l3: numbblock) :=  *)
+
+  Let HBR := fun i1 i2 => happens_before i1 i2 = true.
+  Let HBnum (na1 na2: positive * instruction) := happens_before (snd na1) (snd na2).
+  Let HBGenR (l: list instruction) := GenR HBR l.
+
+
+  (* Data structure to store dependence relation *)
+  Definition DPMap_t := PMap.t (option (instruction * PS.t)).
+
+  (* Definition DPMap_init := PMap.init (option (instruction * S.t)). *)
+  (* Definition DPMap_set := PMap.set (option (instruction * S.t)). *)
+
+  (* Definition depends_on (i1 i2: instruction) := happens_before *)
+
+
+  (* input l should be !!reversed!! list of original list,
+      aka computing from end to head of a block,                                                                                                                                                                                        for efficient definition/computing *)
+  Fixpoint dep_pset (i: instruction) (l_rev: numblock): PS.t :=
+    match l_rev with
+    | nil => PS.empty
+    | (k', i') :: l_rev' => if happens_before i' i 
+                        then PS.add k' (dep_pset i l_rev')
+                        else dep_pset i l_rev'
+    end.
+
+  Fixpoint dep_map (l_rev: numblock): DPMap_t :=
+    match l_rev with
+    | nil => PMap.init None
+    | (k, i) :: l_rev' => PMap.set k (Some (i, dep_pset i l_rev')) (dep_map l_rev')
+    end.
+
+  (* Compute the map that stores the dependence relation inside a basic block *)
+  Definition dep_map_gen (nl: list (positive * instruction)) :=
+    dep_map (List.rev nl).
+
+
+  Lemma dep_map_gen_included:
+   forall l p i ps, (dep_map_gen (numlistgen l)) !! p = Some (i, ps) -> In (p, i) (numlistgen l).
+  Proof.
+
+  Admitted.
+
+  Locate positive. Print positive. Locate Pos.of_nat.
+
+  (* Definition dep_GenRb (l: list instruction) (pi1 pi2: positive * instruction): bool :=
+    let M := dep_map (List.rev (numlistgen l)) in
+    match PMap.get (fst pi1) M with
+    | None => false
+    | Some (i, ps) => PS.mem (fst pi2) ps
+    end. *)
+
+
+  Definition dep_map_gen' (i: positive) (l: list instruction) :=
+    dep_map (List.rev (numlistgen' l i)).
+
+  (* Definition dep_GenRb' (i: positive) (l: list instruction) (pi1 pi2: positive * instruction): bool :=
+    let M := dep_map (List.rev (numlistgen' l i)) in
+    match PMap.get (fst pi1) M with
+    | None => false
+    | Some (i, ps) => PS.mem (fst pi2) ps
+    end. *)
+
+  Inductive dec_numlist: list (positive*instruction) -> Prop :=
+  | dec_numlist_nil: dec_numlist []
+  | dec_numlist_cons: forall pi nl, dec_numlist nl ->
+      (forall pi', In pi' nl -> (fst pi') < (fst pi)) ->
+        dec_numlist (pi::nl)
+  .
+
+  Lemma dep_map_sound_prepare1:
+    forall nl pi1 pi2 i ps, dec_numlist nl -> In pi1 nl -> In pi2 nl -> 
+    let M := dep_map nl in
+      PMap.get (fst pi1) M = Some (i, ps) ->
+        PS.mem (fst pi2) ps = true ->
+          (fst pi2) < (fst pi1).
+  Proof.
+    induction nl.
+    - intros. admit.
+    - intros. simpl in M. destruct a as [p i'].
+    
+
+  Admitted.
+
+
+  Lemma dep_map_sound:
+    forall l k pi1 pi2 i ps, In pi1 (numlistgen' l k) -> In pi2 (numlistgen' l k) -> 
+    let M := dep_map (List.rev (numlistgen' l k)) in
+      PMap.get (fst pi1) M = Some (i, ps) ->
+        PS.mem (fst pi2) ps = true ->
+          GenR' HBR l k pi2 pi1.
+  Proof.
+    (* induction l.
+    - admit.
+    - *)
+    intros. destruct pi1 as [p1 i1]; simpl in H1.
+    destruct pi2 as [p2 i2]; simpl in H2.
+    eapply GenR_intro; eauto; simpl.
+    -
+    admit.
+
+    - unfold HBR.
+
+  Admitted.
+
+  Lemma dep_map_complete:
+  forall l k pi1 pi2,
+  let M := dep_map (List.rev (numlistgen' l k)) in
+    GenR' HBR l k pi1 pi2 ->
+    exists ps, PMap.get (fst pi1) M = Some (snd pi1, ps) /\ PS.mem (fst pi2) ps = true.
+  Proof.
+    (* induction l.
+    - admit.
+    - intros. inv H. *)
+
+    intros. inv H. destruct pi1 as [p1 i1]; simpl in H2, H3.
+    destruct pi2 as [p2 i2]; simpl in H2, H3. simpl.
+
+  Admitted.
+
+  (* Lemma dep_GenRb'_sound:
+    forall l k pi1 pi2, In pi1 (numlistgen' l k) -> In pi2 (numlistgen' l k) -> 
+      dep_GenRb' k l pi1 pi2 = true -> GenR' HBR l k pi1 pi2.
+  Proof.
+    intros. unfold dep_GenRb' in H1. destruct pi1 as [p1 i1]; simpl in H1.
+    remember ((dep_map (rev (numlistgen' l k))) !! p1) as b.
+    destruct b; symmetry in Heqb. 2: discriminate H1.
+    destruct p as [i1' ps]. destruct pi2 as [p2 i2]; simpl in H1.
+    eapply GenR_intro; eauto; simpl.
+    
+ 
+    (* should be fine? *) 
+  Admitted.
+
+  Lemma dep_GenRb'_complete:
+    forall l i pi1 pi2, GenR' HBR l i pi1 pi2 -> dep_GenRb' i l pi1 pi2 = true.
+  Proof.
+    intros. inv H. unfold dep_GenRb'. destruct pi1 as [p1 i1]; simpl.
+    
+
+  Admitted. *)
+
+  (* Lemma dep_GenRb_sound:
+    forall l pi1 pi2, dep_GenRb l pi1 pi2 = true -> GenR HBR l pi1 pi2.
+  Proof. unfold dep_GenRb. intros. eapply dep_GenRb'_sound; eauto. Qed. *)
+
+  Print List.rev.
+
+  (* Generated relation from a basic block *)  
+
+  (* Nodes that are independent, a.k.a ready to be scheduled in current dependence graph
+        a node is empty indicates that it is independent
+          and no other instrucion have to happens before it *)
+  Fixpoint indep_nodes'  (m : PTree.tree' (option (instruction * PS.t))) (i: positive) 
+    (k: list (positive * instruction)) {struct m}: list (positive * instruction) :=
+    match m with
+    | PTree.Node001 r => indep_nodes' r (xI i) k
+    | PTree.Node010 x => 
+        match x with 
+        | Some xp => if PositiveSet.is_empty (snd xp) 
+                     then (PTree.prev i, fst xp) :: k
+                     else k
+        | None => k
+        end
+    | PTree.Node011 x r =>
+        match x with 
+        | Some xp => if PositiveSet.is_empty (snd xp) 
+                     then (PTree.prev i, fst xp) :: indep_nodes' r (xI i) k
+                     else indep_nodes' r (xI i) k
+        | None => indep_nodes' r (xI i) k
+        end
+    | PTree.Node100 l => indep_nodes' l (xO i) k
+    | PTree.Node101 l r => indep_nodes' l (xO i) (indep_nodes' r (xI i) k)
+    | PTree.Node110 l x =>
+        match x with 
+        | Some xp =>  if PositiveSet.is_empty (snd xp) 
+                      then indep_nodes' l (xO i) ((PTree.prev i, fst xp) ::k)
+                      else indep_nodes' l (xO i) k
+        | None => indep_nodes' l (xO i) k
+        end
+    | PTree.Node111 l x r => 
+        match x with 
+        | Some xp =>  if PositiveSet.is_empty (snd xp)
+                      then ((PTree.prev i, fst xp) :: (indep_nodes' r (xI i) k))
+                      else (indep_nodes' r (xI i) k)
+        | None => indep_nodes' l (xO i) k
+        end
+    end.
+
+  Definition indep_nodes (m : DPMap_t): list (positive * instruction) := 
+    match snd m with 
+    | PTree.Empty => nil 
+    | PTree.Nodes m' => indep_nodes' m' xH nil 
+    end.
+
+  Print option_map.
+
+  Definition remove_node0 (p: positive) (node: option (instruction * PS.t)) :=
+    match node with
+    | Some (i, ps) => Some (i, PS.remove p ps) 
+    | None => None
+    end.
+
+  Definition remove_node (p: positive) (m: DPMap_t): DPMap_t :=
+    (fst m, PTree.map1 (remove_node0 p) (PTree.remove p (snd m))).
+
+  (* return the one to schedule and the new dependence relation after removing it *)
+  Definition schedule_1 (prior: list positive) (original: DPMap_t)
+    (scheduled: list (positive * instruction)) (remain: DPMap_t)
+     : res (list (positive * instruction) * DPMap_t) :=
+  let available := indep_nodes remain in
+    do pi <- firstpick available;
+    OK (scheduled ++ [pi], remove_node (fst pi) remain).
+   
+  Fixpoint schedule_n (prior: list positive) (L: nat) (original: DPMap_t)
+    (scheduled: list (positive * instruction)) (remain: DPMap_t)
+      : res (list (positive * instruction) * DPMap_t) :=
+    match L with
+    | O => OK (scheduled, remain)
+    | Datatypes.S L' => 
+        do (scheduled', remain') <- schedule_1 prior original scheduled remain;
+        schedule_n prior L' original scheduled' remain'  (* TODO *)
+    end.
+  
+  Definition schedule_numblock (nl: list (positive * instruction)) :=
+  let m := dep_map_gen nl in
+  let prior := prioritizer (numlistoff nl) in
+    do (nl', m) <- schedule_n prior (List.length nl) m [] m;
+    OK nl'.
+
+  (* Can test compiler using this function without finishing proof *)
+  Definition list_schedule' := schedule_program schedule_numblock.
+
+
+
+  Lemma remove_node_submap: 
+  forall m p1 p2 i2 ps2, (remove_node p1 m) !! p2 = Some (i2, ps2) ->
+    m !! p2 = Some (i2, ps2).
+  Proof.
+    intros. unfold remove_node in H.
+  Admitted.
+
+
+  Inductive schedule_invariant
+    (* (original: list instruction) (originaln := numlistgen original)
+    (scheduled: list (positive * instruction))  (remain: DPMap_t) *)
+    (l: list instruction) (original: DPMap_t)
+    (scheduled: list (positive * instruction)) (remain: DPMap_t)
+    : Prop := 
+    | sched_inv_intro
+      (L2MAP: original = dep_map_gen (numlistgen l))
+      (EXCLUSIVE1: forall p i, List.In (p, i) scheduled -> PMap.get p remain = None)
+      (EXCLUSIVE2: forall p i ps, PMap.get p remain = Some (i, ps) -> ~ List.In (p, i) scheduled)
+      (SUBMAP: forall p i ps, PMap.get p remain = Some (i, ps) ->
+        exists ps', PMap.get p original = Some (i, ps') /\ True ) (* TODO: subset relation *)
+      (SUBLIST: forall p i, List.In (p, i) scheduled -> exists ps, PMap.get p original = Some (i, ps) )
+      (INCL: forall p i ps, PMap.get p original = Some (i, ps) -> 
+                PMap.get p remain = Some (i, ps) \/ List.In (p, i) scheduled)
+      (NODUP: NoDup scheduled)
+      (SORT': forall p1 i1 p2 i2 ps2, In (p1, i1) scheduled -> remain !! p2 = Some (i2, ps2) ->
+                 ~ GenR HBR l (p2, i2) (p1, i1) )
+      (SORT: tsorted HBR l scheduled) 
+      (* (SORT: forall p1 i1 p2 i2 ps2, List.In (p1, i1) scheduled ->  PMap.get p2 remain = Some (i2, ps2) ->
+               True )  *)
+               (* TODO *)
+      :
+      schedule_invariant l original scheduled remain
+  .
+
+  Lemma initial_invariant_preserve:
+    forall l, let original := dep_map_gen (numlistgen l) in
+      schedule_invariant l original [] original.
+  Proof.
+    intros. apply sched_inv_intro.
+    - auto.
+    - intros. destruct H.
+    - intros. intro. destruct H0.
+    - intros. exists ps. auto. (* TODO *)
+    - intros. destruct H.
+    - intros; auto.
+    - intros; auto. eapply NoDup_nil.
+    - intros. destruct H.
+    - eapply topo_sorted_nil.
+  Qed.
+
+  Lemma schedule_1_invariant_preserve:
+    forall prior l original scheduled remain scheduled' remain',
+      schedule_1 prior original scheduled remain = OK (scheduled', remain') -> 
+        schedule_invariant l original scheduled remain ->
+          schedule_invariant l original scheduled' remain'.
+  Proof.
+    intros. inv H0. eapply sched_inv_intro.
+    - auto.
+    (* EXCLUSIVE1 *)
+    - monadInv H. intros.
+      eapply in_app_or in H; destruct H.
+      eapply EXCLUSIVE1 in H. admit. (* fine *)
+      destruct H. subst. simpl. admit. (* fine *)
+      destruct H.
+    (* EXCLUSIVE2 *)
+    - monadInv H.  intros.
+
+      admit.
+    
+    (* SUBMAP *)
+    - admit.
+
+    (* SUBLIST *)
+    - intros. monadInv H. eapply in_app_or in H0. destruct H0; auto.
+      simpl in H. destruct H. subst. 
+      assert(exists ps, remain !! p = Some (i, ps)).
+      { admit. } destruct H.
+      eapply SUBMAP in H. destruct H. destruct H. exists x0; auto.
+      destruct H.
+    
+    (* INCL *)
+    - admit. (* TODO maybe useless*)
+
+    (* NODUP *)
+    - monadInv H. destruct x as [p i].
+      assert(NoDup_swap: forall (A: Type) (l1 l2: list A), NoDup (l1 ++ l2) -> NoDup (l2++l1)).
+      { admit. }
+      eapply NoDup_swap. eapply NoDup_cons; auto.
+      eapply firstpick_sound in EQ.
+      admit. (* fine? *)
+    
+    (* SORT' *)
+    - intros. monadInv H. eapply in_app_or in H0. destruct H0.
+      { eapply SORT'; auto. admit. (* pretty fine! *) }
+      { simpl in H. destruct H. 2: { destruct H. } subst. simpl in H1.
+        eapply firstpick_sound in EQ. admit.   }
+
+    (* SORT *)
+    - monadInv H. eapply topo_soerted_app; eauto. intros. destruct a as [p i].
+      
+    admit.
+  Admitted.
+
+  Lemma schedule_n_invariant_preserve:
+    forall prior L l original scheduled remain scheduled' remain',
+      schedule_n prior L original scheduled remain = OK (scheduled', remain') -> 
+        schedule_invariant l original scheduled remain ->
+          schedule_invariant l original scheduled' remain'.
+  Proof.
+    induction L; intros. monadInv H; auto.
+    simpl in H. monadInv H. eapply IHL; eauto.
+    eapply schedule_1_invariant_preserve; eauto.
+  Qed.
+
+  Lemma final_invariant_preserve:
+    forall prior l scheduled' remain',
+    let original := dep_map_gen (numlistgen l) in
+    let L := length l in
+      schedule_n prior L original [] original = OK (scheduled', remain') ->
+        schedule_invariant l original scheduled' remain'.
+  Proof.
+    intros. eapply schedule_n_invariant_preserve; eauto.
+    eapply initial_invariant_preserve.
+  Qed.
+
+
+  Lemma schedule_1_length_1:
+  forall prior original scheduled remain scheduled' remain',
+    schedule_1 prior original scheduled remain = OK (scheduled', remain') ->
+      length scheduled' = Datatypes.S (length scheduled).
+  Proof. intros. monadInv H. rewrite app_length. simpl. lia. Qed.
+
+  Lemma schedule_n_length_n:
+    forall prior L original scheduled remain scheduled' remain',
+      schedule_n prior L original scheduled remain = OK (scheduled', remain') ->
+        length scheduled' = Nat.add L (length scheduled).
+  Proof.
+    induction L; intros.
+    - simpl in H. inv H. auto.
+    - simpl in H. monadInv H. eapply IHL in EQ0. rewrite EQ0.
+      eapply schedule_1_length_1 in EQ. rewrite EQ. lia.
+  Qed.
+
+  Lemma schedule_original_length:
+    forall prior L original scheduled' remain',
+      schedule_n prior L original [] original = OK (scheduled', remain') ->
+        length scheduled' = L.
+  Proof. intros. eapply schedule_n_length_n in H. simpl in H. lia. Qed. 
+
+
+  Lemma schedule_numblock_correct:
+    forall l nl', schedule_numblock (numlistgen l) = OK nl' ->
+      treorder HBR l (numlistgen l) nl'.
+  Proof.
+    intros. monadInv H. erewrite <- numlistgen_length in EQ.
+    eapply final_invariant_preserve in EQ as INV.
+    eapply sorted_same_elements_topo_reorder.
+    - set(nl := numlistgen l).
+      eapply SameLength_NoDupSame; eauto.
+      { eapply schedule_original_length in EQ; auto. admit. }
+      { eapply numlistgen_NoDup. }
+      { inv INV; eapply NODUP. }
+      { inv INV. intro; intros. destruct a as [p i].
+        eapply SUBLIST in H as ?. destruct H0. eapply dep_map_gen_included; eauto. }
+    - eapply tsorted_self.
+    -
+
+  Admitted.
+
+  Theorem abstract_list_schedule_forward_simulation:
+    forall prog tprog, list_schedule' prog = OK tprog -> 
+      forward_simulation (Linear.semantics prog) (Linear.semantics tprog).
+  Proof.
+    intros. eapply schedule_program_forward_simulation; eauto.
+    eapply schedule_numblock_correct.
+  Qed.
+
+
+
+
+  (* Lemma schedule_block_topo_reorder: *)
+
+
+
+
+  Print PTree.map.
+
+End ABSTRACT_LIST_SCHEDULER.
+
+
+
+
+
+
+
+
+
+
+Check list_schedule'.
+
 Require Import ExtrOcamlIntConv.
+Parameter prioritizer : list int -> int -> list (list int) -> int -> (list int).
 
-Parameter prioritizer : list int -> int -> list (list int) -> int -> unit.
+Locate instruction.
 
-Definition schedule := prioritizer.
+(* TODO : define a convert table *)
+Definition inst2id (i: instruction): positive := 1.
+
+Definition block2ids (l: list instruction): list int :=
+  List.map (compose int_of_pos inst2id) l.
+
+Fixpoint inst2edges (pi: positive * instruction) 
+  (nl: list (positive * instruction)): list (list int) :=
+  match nl with
+  | nil => nil
+  | pi' :: nl' => if happens_before (snd pi) (snd pi') 
+                  then [int_of_pos (fst pi); int_of_pos (fst pi')] :: inst2edges pi nl'
+                  else inst2edges pi nl'
+  end.
+
+Fixpoint nblock2edges (nl: list (positive * instruction)): list (list int) :=
+  match nl with
+  | nil => nil
+  | pi :: nl' => (inst2edges pi nl') ++ nblock2edges nl'
+  end.
+
+Definition prioritizer' (l: list instruction): list positive :=
+  let nodes := block2ids l in
+  let edges := nblock2edges (numlistgen l) in
+  let prior' :=
+    prioritizer
+      nodes (int_of_nat (length nodes))
+      edges (int_of_nat (length edges)) in
+   List.map pos_of_int prior'   
+  .
+
+
+Definition transf_program := list_schedule' prioritizer'.
+
+Check match_prog.
+
+Theorem list_schedule_forward_simulation:
+forall prog tprog, transf_program prog = OK tprog -> 
+  forward_simulation (Linear.semantics prog) (Linear.semantics tprog).
+Proof.
+  intros. eapply abstract_list_schedule_forward_simulation; eauto.
+Qed.
